@prefix airo: <https://w3id.org/airo#> .
@prefix dcterms: <http://purl.org/dc/terms/> .
@prefix linkml: <https://w3id.org/linkml/> .
@prefix nexus: <https://ibm.github.io/risk-atlas-nexus/ontology/> .
@prefix owl: <http://www.w3.org/2002/07/owl#> .
@prefix pav: <http://purl.org/pav/> .
@prefix rdf: <http://www.w3.org/1999/02/22-rdf-syntax-ns#> .
@prefix rdfs: <http://www.w3.org/2000/01/rdf-schema#> .
@prefix skos: <http://www.w3.org/2004/02/skos/core#> .
@prefix xsd: <http://www.w3.org/2001/XMLSchema#> .

nexus:AiAgent a owl:Class ;
    rdfs:label "AiAgent" ;
    rdfs:subClassOf [ a owl:Restriction ;
            owl:allValuesFrom owl:Thing ;
            owl:onProperty nexus:isProvidedBy ],
        [ a owl:Restriction ;
            owl:maxCardinality 1 ;
            owl:onProperty nexus:isProvidedBy ],
        [ a owl:Restriction ;
            owl:minCardinality 0 ;
            owl:onProperty nexus:isProvidedBy ],
        nexus:AiSystem ;
    skos:definition "An artificial intelligence (AI) agent refers to a system or program that is capable of autonomously performing tasks on behalf of a user or another system by designing its workflow and utilizing available tools." ;
    skos:inScheme nexus:ai_system .

nexus:AiOffice a owl:Class ;
    rdfs:label "AiOffice" ;
    rdfs:subClassOf nexus:Organization ;
    skos:definition "The EU AI Office (https://digital-strategy.ec.europa.eu/en/policies/ai-office)" ;
    skos:exactMatch <http://schema.org/Organization> ;
    skos:inScheme nexus:eu_ai_act .

nexus:Container a owl:Class ;
    rdfs:label "Container" ;
    rdfs:subClassOf [ a owl:Restriction ;
            owl:minCardinality 0 ;
            owl:onProperty nexus:stakeholdergroups ],
        [ a owl:Restriction ;
            owl:minCardinality 0 ;
            owl:onProperty nexus:riskcontrols ],
        [ a owl:Restriction ;
            owl:minCardinality 0 ;
            owl:onProperty nexus:datasets ],
        [ a owl:Restriction ;
            owl:allValuesFrom nexus:LargeLanguageModel ;
            owl:onProperty nexus:aimodels ],
        [ a owl:Restriction ;
            owl:allValuesFrom nexus:RiskIncident ;
            owl:onProperty nexus:riskincidents ],
        [ a owl:Restriction ;
            owl:minCardinality 0 ;
            owl:onProperty nexus:licenses ],
        [ a owl:Restriction ;
            owl:minCardinality 0 ;
            owl:onProperty nexus:risks ],
        [ a owl:Restriction ;
            owl:allValuesFrom nexus:AiTask ;
            owl:onProperty nexus:aitasks ],
        [ a owl:Restriction ;
            owl:minCardinality 0 ;
            owl:onProperty nexus:aievalresults ],
        [ a owl:Restriction ;
            owl:minCardinality 0 ;
            owl:onProperty nexus:documents ],
        [ a owl:Restriction ;
            owl:minCardinality 0 ;
            owl:onProperty nexus:llmintrinsics ],
        [ a owl:Restriction ;
            owl:minCardinality 0 ;
            owl:onProperty nexus:adapters ],
        [ a owl:Restriction ;
            owl:minCardinality 0 ;
            owl:onProperty nexus:aimodels ],
        [ a owl:Restriction ;
            owl:allValuesFrom nexus:License ;
            owl:onProperty nexus:licenses ],
        [ a owl:Restriction ;
            owl:minCardinality 0 ;
            owl:onProperty nexus:riskgroups ],
        [ a owl:Restriction ;
            owl:allValuesFrom nexus:LLMIntrinsic ;
            owl:onProperty nexus:llmintrinsics ],
        [ a owl:Restriction ;
            owl:minCardinality 0 ;
            owl:onProperty nexus:evaluations ],
        [ a owl:Restriction ;
            owl:allValuesFrom nexus:LargeLanguageModelFamily ;
            owl:onProperty nexus:aimodelfamilies ],
        [ a owl:Restriction ;
            owl:allValuesFrom nexus:BenchmarkMetadataCard ;
            owl:onProperty nexus:benchmarkmetadatacards ],
        [ a owl:Restriction ;
            owl:allValuesFrom nexus:AiEval ;
            owl:onProperty nexus:evaluations ],
        [ a owl:Restriction ;
            owl:minCardinality 0 ;
            owl:onProperty nexus:organizations ],
        [ a owl:Restriction ;
            owl:allValuesFrom nexus:Organization ;
            owl:onProperty nexus:organizations ],
        [ a owl:Restriction ;
            owl:minCardinality 0 ;
            owl:onProperty nexus:aimodelfamilies ],
        [ a owl:Restriction ;
            owl:allValuesFrom nexus:Term ;
            owl:onProperty nexus:terms ],
        [ a owl:Restriction ;
            owl:minCardinality 0 ;
            owl:onProperty nexus:aitasks ],
        [ a owl:Restriction ;
            owl:allValuesFrom nexus:Risk ;
            owl:onProperty nexus:risks ],
        [ a owl:Restriction ;
            owl:allValuesFrom nexus:StakeholderGroup ;
            owl:onProperty nexus:stakeholdergroups ],
        [ a owl:Restriction ;
            owl:allValuesFrom nexus:Vocabulary ;
            owl:onProperty nexus:vocabularies ],
        [ a owl:Restriction ;
            owl:allValuesFrom nexus:Action ;
            owl:onProperty nexus:actions ],
        [ a owl:Restriction ;
            owl:allValuesFrom nexus:Stakeholder ;
            owl:onProperty nexus:stakeholders ],
        [ a owl:Restriction ;
            owl:minCardinality 0 ;
            owl:onProperty nexus:taxonomies ],
        [ a owl:Restriction ;
            owl:minCardinality 0 ;
            owl:onProperty nexus:terms ],
        [ a owl:Restriction ;
            owl:allValuesFrom nexus:AiEvalResult ;
            owl:onProperty nexus:aievalresults ],
        [ a owl:Restriction ;
            owl:allValuesFrom nexus:Modality ;
            owl:onProperty nexus:modalities ],
        [ a owl:Restriction ;
            owl:minCardinality 0 ;
            owl:onProperty nexus:vocabularies ],
        [ a owl:Restriction ;
            owl:allValuesFrom nexus:Dataset ;
            owl:onProperty nexus:datasets ],
        [ a owl:Restriction ;
            owl:minCardinality 0 ;
            owl:onProperty nexus:actions ],
        [ a owl:Restriction ;
            owl:allValuesFrom nexus:Documentation ;
            owl:onProperty nexus:documents ],
        [ a owl:Restriction ;
            owl:minCardinality 0 ;
            owl:onProperty nexus:modalities ],
        [ a owl:Restriction ;
            owl:allValuesFrom nexus:RiskControl ;
            owl:onProperty nexus:riskcontrols ],
        [ a owl:Restriction ;
            owl:minCardinality 0 ;
            owl:onProperty nexus:stakeholders ],
        [ a owl:Restriction ;
            owl:minCardinality 0 ;
            owl:onProperty nexus:riskincidents ],
        [ a owl:Restriction ;
            owl:allValuesFrom nexus:Adapter ;
            owl:onProperty nexus:adapters ],
        [ a owl:Restriction ;
            owl:allValuesFrom nexus:RiskGroup ;
            owl:onProperty nexus:riskgroups ],
        [ a owl:Restriction ;
            owl:allValuesFrom nexus:RiskTaxonomy ;
            owl:onProperty nexus:taxonomies ],
        [ a owl:Restriction ;
            owl:minCardinality 0 ;
            owl:onProperty nexus:benchmarkmetadatacards ] ;
    skos:definition "An umbrella object that holds the ontology class instances" ;
    skos:inScheme nexus:ai-risk-ontology .

nexus:IncidentConcludedclass a owl:Class ;
    rdfs:label "IncidentConcludedclass" ;
    rdfs:subClassOf nexus:IncidentStatus ;
    skos:exactMatch <https://w3id.org/dpv#IncidentConcludedclass> ;
    skos:inScheme nexus:ai_risk .

nexus:IncidentHaltedclass a owl:Class ;
    rdfs:label "IncidentHaltedclass" ;
    rdfs:subClassOf nexus:IncidentStatus ;
    skos:exactMatch <https://w3id.org/dpv#IncidentHaltedclass> ;
    skos:inScheme nexus:ai_risk .

nexus:IncidentMitigatedclass a owl:Class ;
    rdfs:label "IncidentMitigatedclass" ;
    rdfs:subClassOf nexus:IncidentStatus ;
    skos:exactMatch <https://w3id.org/dpv#IncidentMitigatedclass> ;
    skos:inScheme nexus:ai_risk .

nexus:IncidentNearMissclass a owl:Class ;
    rdfs:label "IncidentNearMissclass" ;
    rdfs:subClassOf nexus:IncidentStatus ;
    skos:exactMatch <https://w3id.org/dpv#IncidentNearMissclass> ;
    skos:inScheme nexus:ai_risk .

nexus:IncidentOngoingclass a owl:Class ;
    rdfs:label "IncidentOngoingclass" ;
    rdfs:subClassOf nexus:IncidentStatus ;
    skos:exactMatch <https://w3id.org/dpv#IncidentOngoingclass> ;
    skos:inScheme nexus:ai_risk .

nexus:Input a owl:Class ;
    rdfs:label "Input" ;
    rdfs:subClassOf nexus:Entity ;
    skos:definition "Input for which the system or component generates output." ;
    skos:exactMatch airo:Input ;
    skos:inScheme nexus:ai_system .

nexus:Principle a owl:Class ;
    rdfs:label "Principle" ;
    skos:definition "A representation of values or norms that must be taken into consideration when conducting activities" ;
    skos:exactMatch <https://w3id.org/dpv#Principle> ;
    skos:inScheme nexus:common .

nexus:Questionnaire a owl:Class ;
    rdfs:label "Questionnaire" ;
    rdfs:subClassOf [ a owl:Restriction ;
            owl:maxCardinality 1 ;
            owl:onProperty nexus:composed_of ],
        [ a owl:Restriction ;
            owl:minCardinality 0 ;
            owl:onProperty nexus:composed_of ],
        [ a owl:Restriction ;
            owl:allValuesFrom nexus:Question ;
            owl:onProperty nexus:composed_of ],
        nexus:AiEval ;
    skos:definition "A questionnaire groups questions" ;
    skos:inScheme nexus:ai_eval .

nexus:ai-risk-ontology.owl.ttl a owl:Ontology ;
    rdfs:label "ai-risk-ontology" ;
    dcterms:license "https://www.apache.org/licenses/LICENSE-2.0.html" ;
    pav:version "0.5.0" ;
    skos:definition "An ontology describing AI systems and their risks" .

nexus:hasTerm a owl:ObjectProperty ;
    rdfs:label "hasTerm" ;
    rdfs:range nexus:Term ;
    skos:definition "Indicates terms associated with a vocabulary" ;
    skos:inScheme nexus:common .

nexus:isDeployedBy a owl:ObjectProperty ;
    rdfs:label "isDeployedBy" ;
    rdfs:range nexus:Organization ;
    skos:definition "A relationship indicating that an entity has been deployed by an organization." ;
    skos:inScheme nexus:eu_ai_act .

nexus:isDistributedBy a owl:ObjectProperty ;
    rdfs:label "isDistributedBy" ;
    rdfs:range nexus:Organization ;
    skos:definition "A relationship indicating that an entity has been distributed by an organization." ;
    skos:inScheme nexus:eu_ai_act .

nexus:isImportedBy a owl:ObjectProperty ;
    rdfs:label "isImportedBy" ;
    rdfs:range nexus:Organization ;
    skos:definition "A relationship indicating that an entity has been imported by an organization." ;
    skos:inScheme nexus:eu_ai_act .

nexus:training_data_preprocessing a owl:ObjectProperty ;
    rdfs:label "training_data_preprocessing" ;
    rdfs:range nexus:DataPreprocessing ;
    skos:definition "relationship indicating data preprocessing steps performed on training data sets to ensure high quality training data." ;
    skos:inScheme nexus:ai_system .

nexus:validated_by a owl:ObjectProperty ;
    rdfs:label "validated_by" ;
    rdfs:range nexus:AiModelValidation ;
    skos:definition "A relationship indicating the model validation steps after AI model training." ;
    skos:inScheme nexus:ai_system .

nexus:AiModel a owl:Class ;
    rdfs:label "AiModel" ;
    rdfs:subClassOf [ a owl:Restriction ;
            owl:allValuesFrom xsd:string ;
            owl:onProperty nexus:architecture ],
        [ a owl:Restriction ;
            owl:maxCardinality 1 ;
            owl:onProperty nexus:architecture ],
        [ a owl:Restriction ;
            owl:allValuesFrom nexus:RiskControl ;
            owl:onProperty nexus:hasRiskControl ],
        [ a owl:Restriction ;
            owl:maxCardinality 1 ;
            owl:onProperty nexus:carbon_emitted ],
        [ a owl:Restriction ;
            owl:minCardinality 0 ;
            owl:onProperty nexus:power_consumption_w ],
        [ a owl:Restriction ;
            owl:minCardinality 0 ;
            owl:onProperty nexus:carbon_emitted ],
        [ a owl:Restriction ;
            owl:minCardinality 0 ;
            owl:onProperty nexus:architecture ],
        [ a owl:Restriction ;
            owl:allValuesFrom nexus:AiEvalResult ;
            owl:onProperty nexus:hasEvaluation ],
        [ a owl:Restriction ;
            owl:minCardinality 0 ;
            owl:onProperty nexus:gpu_hours ],
        [ a owl:Restriction ;
            owl:maxCardinality 1 ;
            owl:onProperty nexus:power_consumption_w ],
        [ a owl:Restriction ;
            owl:minCardinality 0 ;
            owl:onProperty nexus:hasRiskControl ],
        [ a owl:Restriction ;
            owl:allValuesFrom [ a rdfs:Datatype ;
                    owl:intersectionOf ( xsd:integer [ a rdfs:Datatype ;
                                owl:onDatatype xsd:integer ;
                                owl:withRestrictions ( [ xsd:minInclusive 0 ] ) ] ) ] ;
            owl:onProperty nexus:power_consumption_w ],
        [ a owl:Restriction ;
            owl:allValuesFrom [ a rdfs:Datatype ;
                    owl:intersectionOf ( xsd:integer [ a rdfs:Datatype ;
                                owl:onDatatype xsd:integer ;
                                owl:withRestrictions ( [ xsd:minInclusive 0 ] ) ] ) ] ;
            owl:onProperty nexus:gpu_hours ],
        [ a owl:Restriction ;
            owl:maxCardinality 1 ;
            owl:onProperty nexus:gpu_hours ],
        [ a owl:Restriction ;
            owl:allValuesFrom [ a rdfs:Datatype ;
                    owl:intersectionOf ( xsd:float [ a rdfs:Datatype ;
                                owl:onDatatype xsd:integer ;
                                owl:withRestrictions ( [ xsd:minInclusive 0 ] ) ] ) ] ;
            owl:onProperty nexus:carbon_emitted ],
        [ a owl:Restriction ;
            owl:minCardinality 0 ;
            owl:onProperty nexus:hasEvaluation ],
        nexus:BaseAi ;
    skos:definition "A base AI Model class. No assumption about the type (SVM, LLM, etc.). Subclassed by model types (see LargeLanguageModel)." ;
    skos:inScheme nexus:ai_system .

nexus:AiModelValidation a owl:Class ;
    rdfs:label "AiModelValidation" ;
    rdfs:subClassOf nexus:AiLifecyclePhase ;
    skos:definition "AI model validation steps that have been performed after the model training to ensure high AI model quality." ;
    skos:inScheme nexus:ai_system .

nexus:AiSystem a owl:Class ;
    rdfs:label "AiSystem" ;
    rdfs:subClassOf [ a owl:Restriction ;
            owl:allValuesFrom nexus:EuAiRiskCategory ;
            owl:onProperty nexus:hasEuRiskCategory ],
        [ a owl:Restriction ;
            owl:minCardinality 0 ;
            owl:onProperty nexus:isComposedOf ],
        [ a owl:Restriction ;
            owl:maxCardinality 1 ;
            owl:onProperty nexus:hasEuRiskCategory ],
        [ a owl:Restriction ;
            owl:allValuesFrom nexus:BaseAi ;
            owl:onProperty nexus:isComposedOf ],
        [ a owl:Restriction ;
            owl:minCardinality 0 ;
            owl:onProperty nexus:hasEuRiskCategory ],
        [ a owl:Restriction ;
            owl:allValuesFrom nexus:AiSystemType ;
            owl:onProperty nexus:hasEuAiSystemType ],
        [ a owl:Restriction ;
            owl:minCardinality 0 ;
            owl:onProperty nexus:hasEuAiSystemType ],
        [ a owl:Restriction ;
            owl:maxCardinality 1 ;
            owl:onProperty nexus:hasEuAiSystemType ],
        nexus:BaseAi ;
    skos:definition "A compound AI System composed of one or more AI capablities. ChatGPT is an example of an AI system which deploys multiple GPT AI models." ;
    skos:exactMatch airo:AISystem ;
    skos:inScheme nexus:ai_system .

nexus:DataPreprocessing a owl:Class ;
    rdfs:label "DataPreprocessing" ;
    rdfs:subClassOf nexus:AiLifecyclePhase ;
    skos:definition "Data transformations, such as PI filtering, performed to ensure high quality of AI model training data." ;
    skos:inScheme nexus:ai_system .

nexus:Fact a owl:Class ;
    rdfs:label "Fact" ;
    rdfs:subClassOf [ a owl:Restriction ;
            owl:minCardinality 0 ;
            owl:onProperty nexus:evidence ],
        [ a owl:Restriction ;
            owl:maxCardinality 1 ;
            owl:onProperty nexus:evidence ],
        [ a owl:Restriction ;
            owl:maxCardinality 1 ;
            owl:onProperty nexus:value ],
        [ a owl:Restriction ;
            owl:allValuesFrom xsd:string ;
            owl:onProperty nexus:value ],
        [ a owl:Restriction ;
            owl:allValuesFrom xsd:string ;
            owl:onProperty nexus:evidence ],
        [ a owl:Restriction ;
            owl:minCardinality 1 ;
            owl:onProperty nexus:value ] ;
    skos:definition "A fact about something, for example the result of a measurement. In addition to the value, evidence is provided." ;
    skos:exactMatch <http://schema.org/Statement> ;
    skos:inScheme nexus:common .

nexus:Question a owl:Class ;
    rdfs:label "Question" ;
    rdfs:subClassOf [ a owl:Restriction ;
            owl:allValuesFrom xsd:string ;
            owl:onProperty nexus:text ],
        [ a owl:Restriction ;
            owl:maxCardinality 1 ;
            owl:onProperty nexus:text ],
        [ a owl:Restriction ;
            owl:minCardinality 1 ;
            owl:onProperty nexus:text ],
        nexus:AiEval ;
    skos:definition "An evaluation where a question has to be answered" ;
    skos:inScheme nexus:ai_eval .

nexus:Stakeholder a owl:Class ;
    rdfs:label "Stakeholder" ;
    rdfs:subClassOf [ a owl:Restriction ;
            owl:allValuesFrom nexus:StakeholderGroup ;
            owl:onProperty nexus:isPartOf ],
        [ a owl:Restriction ;
            owl:allValuesFrom nexus:RiskTaxonomy ;
            owl:onProperty nexus:isDefinedByTaxonomy ],
        [ a owl:Restriction ;
            owl:minCardinality 0 ;
            owl:onProperty nexus:isDefinedByTaxonomy ],
        [ a owl:Restriction ;
            owl:maxCardinality 1 ;
            owl:onProperty nexus:isPartOf ],
        [ a owl:Restriction ;
            owl:maxCardinality 1 ;
            owl:onProperty nexus:isDefinedByTaxonomy ],
        [ a owl:Restriction ;
            owl:minCardinality 0 ;
            owl:onProperty nexus:isPartOf ],
        nexus:Entity ;
    skos:definition "An AI system stakeholder for Responsible AI governance (e.g., AI governors, users, consumers)." ;
    skos:inScheme nexus:ai_csiro_rai .

<https://ibm.github.io/risk-atlas-nexus/ontology/AdapterType#ALORA> a owl:Class ;
    rdfs:label "ALORA" ;
    rdfs:subClassOf nexus:AdapterType .

<https://ibm.github.io/risk-atlas-nexus/ontology/AdapterType#LORA> a owl:Class ;
    rdfs:label "LORA" ;
    rdfs:subClassOf nexus:AdapterType .

<https://ibm.github.io/risk-atlas-nexus/ontology/AdapterType#X-LORA> a owl:Class ;
    rdfs:label "X-LORA" ;
    rdfs:subClassOf nexus:AdapterType .

nexus:AiLifecyclePhase a owl:Class ;
    rdfs:label "AiLifecyclePhase" ;
    rdfs:subClassOf nexus:Entity ;
    skos:definition "A Phase of AI lifecycle which indicates evolution of the system from conception through retirement." ;
    skos:exactMatch airo:AILifecyclePhase ;
    skos:inScheme nexus:ai_system .

nexus:AiProvider a owl:Class ;
    rdfs:label "AiProvider" ;
    rdfs:subClassOf nexus:Organization ;
    skos:definition "A provider under the AI Act is defined by Article 3(3) as a natural or legal person or body that develops an AI system or general-purpose AI model or has an AI system or general-purpose AI model developed; and places that system or model on the market, or puts that system into service, under the provider's own name or trademark, whether for payment or free for charge." ;
    skos:exactMatch airo:AIProvider ;
    skos:inScheme nexus:ai_system .

<https://ibm.github.io/risk-atlas-nexus/ontology/AiSystemType#GPAI> a owl:Class ;
    rdfs:label "GPAI" ;
    rdfs:subClassOf nexus:AiSystemType .

<https://ibm.github.io/risk-atlas-nexus/ontology/AiSystemType#GPAI_OS> a owl:Class ;
    rdfs:label "GPAI_OS" ;
    rdfs:subClassOf nexus:AiSystemType .

<https://ibm.github.io/risk-atlas-nexus/ontology/AiSystemType#HIGH_RISK> a owl:Class ;
    rdfs:label "HIGH_RISK" ;
    rdfs:subClassOf nexus:AiSystemType .

<https://ibm.github.io/risk-atlas-nexus/ontology/AiSystemType#MILITARY_SECURITY> a owl:Class ;
    rdfs:label "MILITARY_SECURITY" ;
    rdfs:subClassOf nexus:AiSystemType .

<https://ibm.github.io/risk-atlas-nexus/ontology/AiSystemType#PROHIBITED> a owl:Class ;
    rdfs:label "PROHIBITED" ;
    rdfs:subClassOf nexus:AiSystemType .

<https://ibm.github.io/risk-atlas-nexus/ontology/AiSystemType#SCIENTIFIC_RD> a owl:Class ;
    rdfs:label "SCIENTIFIC_RD" ;
    rdfs:subClassOf nexus:AiSystemType .

nexus:Consequence a owl:Class ;
    rdfs:label "Consequence" ;
    rdfs:subClassOf nexus:Entity ;
    skos:exactMatch <https://w3id.org/dpv#Consequence> ;
    skos:inScheme nexus:ai_risk .

<https://ibm.github.io/risk-atlas-nexus/ontology/EuAiRiskCategory#EXCLUDED> a owl:Class ;
    rdfs:label "EXCLUDED" ;
    rdfs:subClassOf nexus:EuAiRiskCategory .

<https://ibm.github.io/risk-atlas-nexus/ontology/EuAiRiskCategory#HIGH_RISK> a owl:Class ;
    rdfs:label "HIGH_RISK" ;
    rdfs:subClassOf nexus:EuAiRiskCategory .

<https://ibm.github.io/risk-atlas-nexus/ontology/EuAiRiskCategory#HIGH_RISK_EXCEPTION> a owl:Class ;
    rdfs:label "HIGH_RISK_EXCEPTION" ;
    rdfs:subClassOf nexus:EuAiRiskCategory .

<https://ibm.github.io/risk-atlas-nexus/ontology/EuAiRiskCategory#LIMITED_OR_LOW_RISK> a owl:Class ;
    rdfs:label "LIMITED_OR_LOW_RISK" ;
    rdfs:subClassOf nexus:EuAiRiskCategory .

<https://ibm.github.io/risk-atlas-nexus/ontology/EuAiRiskCategory#PROHIBITED> a owl:Class ;
    rdfs:label "PROHIBITED" ;
    rdfs:subClassOf nexus:EuAiRiskCategory .

nexus:LLMIntrinsic a owl:Class ;
    rdfs:label "LLMIntrinsic" ;
    rdfs:subClassOf [ a owl:Restriction ;
            owl:minCardinality 0 ;
            owl:onProperty nexus:hasRelatedTerm ],
        [ a owl:Restriction ;
            owl:minCardinality 0 ;
            owl:onProperty nexus:hasDocumentation ],
        [ a owl:Restriction ;
            owl:allValuesFrom nexus:Adapter ;
            owl:onProperty nexus:hasAdapter ],
        [ a owl:Restriction ;
            owl:minCardinality 0 ;
            owl:onProperty nexus:hasAdapter ],
        [ a owl:Restriction ;
            owl:allValuesFrom nexus:Documentation ;
            owl:onProperty nexus:hasDocumentation ],
        [ a owl:Restriction ;
            owl:minCardinality 0 ;
            owl:onProperty nexus:isDefinedByVocabulary ],
        [ a owl:Restriction ;
            owl:allValuesFrom [ owl:intersectionOf ( [ owl:unionOf ( nexus:RiskConcept nexus:Term ) ] nexus:Term ) ] ;
            owl:onProperty nexus:hasRelatedTerm ],
        [ a owl:Restriction ;
            owl:allValuesFrom nexus:Vocabulary ;
            owl:onProperty nexus:isDefinedByVocabulary ],
        [ a owl:Restriction ;
            owl:maxCardinality 1 ;
            owl:onProperty nexus:isDefinedByVocabulary ],
        [ a owl:Restriction ;
            owl:minCardinality 0 ;
            owl:onProperty nexus:hasRelatedRisk ],
        [ a owl:Restriction ;
            owl:allValuesFrom [ owl:intersectionOf ( [ owl:unionOf ( nexus:RiskConcept nexus:Term ) ] nexus:Risk ) ] ;
            owl:onProperty nexus:hasRelatedRisk ],
        nexus:Entity ;
    skos:definition "A capability that can be invoked through a well-defined API that is reasonably stable and independent of how the LLM intrinsic itself is implemented." ;
    skos:exactMatch <https://w3id.org/dpv/ai#Capability> ;
    skos:inScheme nexus:ai_intrinsic .

nexus:LargeLanguageModelFamily a owl:Class ;
    rdfs:label "LargeLanguageModelFamily" ;
    rdfs:subClassOf [ a owl:Restriction ;
            owl:allValuesFrom nexus:Documentation ;
            owl:onProperty nexus:hasDocumentation ],
        [ a owl:Restriction ;
            owl:minCardinality 0 ;
            owl:onProperty nexus:hasDocumentation ],
        nexus:Entity ;
    skos:definition "A large language model family is a set of models that are provided by the same AI systems provider and are built around the same architecture, but differ e.g. in the number of parameters. Examples are Meta's Llama2 family or the IBM granite models." ;
    skos:inScheme nexus:ai_system .

nexus:Likelihood a owl:Class ;
    rdfs:label "Likelihood" ;
    rdfs:subClassOf nexus:Entity ;
    skos:exactMatch <https://w3id.org/dpv#Likelihood> ;
    skos:inScheme nexus:ai_risk .

nexus:Severity a owl:Class ;
    rdfs:label "Severity" ;
    rdfs:subClassOf nexus:Entity ;
    skos:exactMatch <https://w3id.org/dpv#Severity> ;
    skos:inScheme nexus:ai_risk .

nexus:StakeholderGroup a owl:Class ;
    rdfs:label "StakeholderGroup" ;
    rdfs:subClassOf [ a owl:Restriction ;
            owl:minCardinality 0 ;
            owl:onProperty nexus:isDefinedByTaxonomy ],
        [ a owl:Restriction ;
            owl:maxCardinality 1 ;
            owl:onProperty nexus:isDefinedByTaxonomy ],
        [ a owl:Restriction ;
            owl:allValuesFrom nexus:RiskTaxonomy ;
            owl:onProperty nexus:isDefinedByTaxonomy ],
        nexus:Entity ;
    skos:definition "An AI system stakeholder grouping." ;
    skos:inScheme nexus:ai_csiro_rai .

nexus:actions a owl:ObjectProperty ;
    rdfs:label "actions" ;
    skos:definition "A list of risk related actions" ;
    skos:inScheme nexus:ai-risk-ontology .

nexus:adapters a owl:ObjectProperty ;
    rdfs:label "adapters" ;
    skos:definition "A list of Adapters" ;
    skos:inScheme nexus:ai-risk-ontology .

nexus:aievalresults a owl:ObjectProperty ;
    rdfs:label "aievalresults" ;
    skos:definition "A list of AI evaluation results" ;
    skos:inScheme nexus:ai-risk-ontology .

nexus:aimodelfamilies a owl:ObjectProperty ;
    rdfs:label "aimodelfamilies" ;
    skos:definition "A list of AI model families" ;
    skos:inScheme nexus:ai-risk-ontology .

nexus:aimodels a owl:ObjectProperty ;
    rdfs:label "aimodels" ;
    skos:definition "A list of AI models" ;
    skos:inScheme nexus:ai-risk-ontology .

nexus:aitasks a owl:ObjectProperty ;
    rdfs:label "aitasks" ;
    skos:definition "A list of AI tasks" ;
    skos:inScheme nexus:ai-risk-ontology .

nexus:benchmarkmetadatacards a owl:ObjectProperty ;
    rdfs:label "benchmarkmetadatacards" ;
    skos:definition "A list of AI evaluation benchmark metadata cards" ;
    skos:inScheme nexus:ai-risk-ontology .

nexus:datasets a owl:ObjectProperty ;
    rdfs:label "datasets" ;
    skos:definition "A list of data sets" ;
    skos:inScheme nexus:ai-risk-ontology .

nexus:documents a owl:ObjectProperty ;
    rdfs:label "documents" ;
    skos:definition "A list of documents" ;
    skos:inScheme nexus:ai-risk-ontology .

nexus:evaluations a owl:ObjectProperty ;
    rdfs:label "evaluations" ;
    skos:definition "A list of AI evaluation methods" ;
    skos:inScheme nexus:ai-risk-ontology .

nexus:hasAdapter a owl:ObjectProperty ;
    rdfs:label "hasAdapter" ;
    rdfs:domain nexus:LLMIntrinsic ;
    rdfs:range nexus:Adapter ;
    skos:definition "The Adapter for the intrinsic" ;
    skos:inScheme nexus:ai_intrinsic .

nexus:hasAiActorTask a owl:DatatypeProperty ;
    rdfs:label "hasAiActorTask" ;
    skos:definition "Pertinent AI Actor Tasks for each subcategory. Not every AI Actor Task listed will apply to every suggested action in the subcategory (i.e., some apply to AI development and others apply to AI deployment)." ;
    skos:inScheme nexus:ai_risk .

nexus:hasCalculation a owl:DatatypeProperty ;
    rdfs:label "hasCalculation" ;
    skos:definition "The way metrics are computed based on model outputs and the benchmark data." ;
    skos:inScheme nexus:ai_eval .

nexus:hasDataSource a owl:DatatypeProperty ;
    rdfs:label "hasDataSource" ;
    skos:definition "The origin or source of the data used in the benchmark (e.g., curated datasets, user submissions)." ;
    skos:inScheme nexus:ai_eval .

nexus:hasDataType a owl:DatatypeProperty ;
    rdfs:label "hasDataType" ;
    skos:definition "The type of data used in the benchmark (e.g., text, images, or multi-modal)" ;
    skos:inScheme nexus:ai_eval .

nexus:hasDataset a owl:ObjectProperty ;
    rdfs:label "hasDataset" ;
    rdfs:range nexus:Dataset ;
    skos:definition "A relationship to datasets that are used." ;
    skos:inScheme nexus:common .

nexus:hasDomains a owl:DatatypeProperty ;
    rdfs:label "hasDomains" ;
    skos:definition "The specific domains or areas where the benchmark is applied (e.g., natural language processing,computer vision)." ;
    skos:inScheme nexus:ai_eval .

nexus:hasEvaluation a owl:ObjectProperty ;
    rdfs:label "hasEvaluation" ;
    rdfs:range nexus:AiEvalResult ;
    skos:definition "A relationship indicating that an entity has an AI evaluation result." ;
    skos:inScheme nexus:ai_eval .

nexus:hasImplementation a owl:DatatypeProperty ;
    rdfs:label "hasImplementation" ;
    rdfs:range xsd:anyURI ;
    skos:definition "A relationship to a implementation defining the risk evaluation" ;
    skos:inScheme nexus:ai_eval .

nexus:hasInputModality a owl:ObjectProperty ;
    rdfs:label "hasInputModality" ;
    rdfs:range nexus:Modality ;
    skos:definition "A relationship indicating the input modalities supported by an AI component. Examples include text, image, video." ;
    skos:inScheme nexus:ai_system .

nexus:hasInterpretation a owl:DatatypeProperty ;
    rdfs:label "hasInterpretation" ;
    skos:definition "How users should interpret the scores or results from the metrics." ;
    skos:inScheme nexus:ai_eval .

nexus:hasLanguages a owl:DatatypeProperty ;
    rdfs:label "hasLanguages" ;
    skos:definition "The languages included in the dataset used by the benchmark (e.g., English, multilingual)." ;
    skos:inScheme nexus:ai_eval .

nexus:hasLimitations a owl:DatatypeProperty ;
    rdfs:label "hasLimitations" ;
    skos:definition "Limitations in evaluating or addressing risks, such as gaps in demographic coverage or specific domains." ;
    skos:inScheme nexus:ai_eval .

nexus:hasMethods a owl:DatatypeProperty ;
    rdfs:label "hasMethods" ;
    skos:definition "The evaluation techniques applied within the benchmark." ;
    skos:inScheme nexus:ai_eval .

nexus:hasMetrics a owl:DatatypeProperty ;
    rdfs:label "hasMetrics" ;
    skos:definition "The specific performance metrics used to assess models (e.g., accuracy, F1 score, precision, recall)." ;
    skos:inScheme nexus:ai_eval .

nexus:hasModelCard a owl:DatatypeProperty ;
    rdfs:label "hasModelCard" ;
    rdfs:range xsd:string ;
    skos:definition "A relationship to model card references." ;
    skos:inScheme nexus:ai_system .

nexus:hasOutOfScopeUses a owl:DatatypeProperty ;
    rdfs:label "hasOutOfScopeUses" ;
    skos:definition "Use cases where the benchmark is not designed to be applied and could give misleading results." ;
    skos:inScheme nexus:ai_eval .

nexus:hasOutputModality a owl:ObjectProperty ;
    rdfs:label "hasOutputModality" ;
    rdfs:range nexus:Modality ;
    skos:definition "A relationship indicating the output modalities supported by an AI component. Examples include text, image, video." ;
    skos:inScheme nexus:ai_system .

nexus:hasParentDefinition a owl:ObjectProperty ;
    rdfs:label "hasParentDefinition" ;
    rdfs:range nexus:Term ;
    skos:definition "Indicates parent terms associated with a term" ;
    skos:inScheme nexus:common .

nexus:hasPart a owl:DatatypeProperty ;
    rdfs:label "hasPart" ;
    skos:definition "A relationship where an entity has another entity" ;
    skos:inScheme nexus:common .

nexus:hasRelatedAction a owl:ObjectProperty ;
    rdfs:label "hasRelatedAction" ;
    rdfs:range nexus:Action ;
    skos:definition "A relationship where an entity relates to an action" ;
    skos:inScheme nexus:ai_risk .

nexus:hasRelatedTerm a owl:ObjectProperty ;
    rdfs:label "hasRelatedTerm" ;
    rdfs:domain nexus:Any ;
    rdfs:range [ owl:intersectionOf ( [ owl:unionOf ( nexus:RiskConcept nexus:Term ) ] nexus:Term ) ] ;
    skos:definition "A relationship where an entity relates to a term" ;
    skos:inScheme nexus:common .

nexus:hasResources a owl:DatatypeProperty ;
    rdfs:label "hasResources" ;
    skos:definition "Links to relevant resources, such as repositories or papers related to the benchmark." ;
    skos:inScheme nexus:ai_eval .

nexus:hasRiskControl a owl:ObjectProperty ;
    rdfs:label "hasRiskControl" ;
    rdfs:range nexus:RiskControl ;
    skos:definition "Indicates the control measures associated with a system or component to modify risks." ;
    skos:inScheme nexus:ai_system .

nexus:hasSimilarBenchmarks a owl:DatatypeProperty ;
    rdfs:label "hasSimilarBenchmarks" ;
    skos:definition "Benchmarks that are closely related in terms of goals or data type." ;
    skos:inScheme nexus:ai_eval .

nexus:hasSubDefinition a owl:ObjectProperty ;
    rdfs:label "hasSubDefinition" ;
    rdfs:range nexus:Term ;
    skos:definition "Indicates child terms associated with a term" ;
    skos:inScheme nexus:common .

nexus:hasTrainingData a owl:ObjectProperty ;
    rdfs:label "hasTrainingData" ;
    rdfs:range nexus:Dataset ;
    skos:definition "A relationship indicating the datasets an AI model was trained on." ;
    skos:inScheme nexus:ai_system .

nexus:hasUnitxtCard a owl:DatatypeProperty ;
    rdfs:label "hasUnitxtCard" ;
    rdfs:range xsd:anyURI ;
    skos:definition "A relationship to a Unitxt card defining the risk evaluation" ;
    skos:inScheme nexus:ai_eval .

nexus:hasValidation a owl:DatatypeProperty ;
    rdfs:label "hasValidation" ;
    skos:definition "Measures taken to ensure that the benchmark provides valid and reliable evaluations." ;
    skos:inScheme nexus:ai_eval .

nexus:licenses a owl:ObjectProperty ;
    rdfs:label "licenses" ;
    skos:definition "A list of licenses" ;
    skos:inScheme nexus:ai-risk-ontology .

nexus:llmintrinsics a owl:ObjectProperty ;
    rdfs:label "llmintrinsics" ;
    skos:definition "A list of LLMIntrinsics" ;
    skos:inScheme nexus:ai-risk-ontology .

nexus:modalities a owl:ObjectProperty ;
    rdfs:label "modalities" ;
    skos:definition "A list of AI modalities" ;
    skos:inScheme nexus:ai-risk-ontology .

nexus:organizations a owl:ObjectProperty ;
    rdfs:label "organizations" ;
    skos:definition "A list of organizations" ;
    skos:inScheme nexus:ai-risk-ontology .

nexus:performsTask a owl:ObjectProperty ;
    rdfs:label "performsTask" ;
    rdfs:range nexus:AiTask ;
    skos:definition "relationship indicating the AI tasks an AI model can perform." ;
    skos:inScheme nexus:ai_system .

nexus:refersToRisk a owl:ObjectProperty ;
    rdfs:label "refersToRisk" ;
    rdfs:domain nexus:RiskIncident ;
    rdfs:range nexus:Risk ;
    skos:definition "Indicates the incident (subject) is a materialisation of the indicated risk (object)" ;
    skos:exactMatch <https://w3id.org/dpv#refersToRisk> ;
    skos:inScheme nexus:ai_risk .

nexus:riskcontrols a owl:ObjectProperty ;
    rdfs:label "riskcontrols" ;
    skos:definition "A list of AI risk controls" ;
    skos:inScheme nexus:ai-risk-ontology .

nexus:riskgroups a owl:ObjectProperty ;
    rdfs:label "riskgroups" ;
    skos:definition "A list of AI risk groups" ;
    skos:inScheme nexus:ai-risk-ontology .

nexus:riskincidents a owl:ObjectProperty ;
    rdfs:label "riskincidents" ;
    skos:definition "A list of AI risk incidents" ;
    skos:inScheme nexus:ai-risk-ontology .

nexus:risks a owl:ObjectProperty ;
    rdfs:label "risks" ;
    skos:definition "A list of AI risks" ;
    skos:inScheme nexus:ai-risk-ontology .

nexus:stakeholdergroups a owl:ObjectProperty ;
    rdfs:label "stakeholdergroups" ;
    skos:definition "A list of AI stakeholder groups" ;
    skos:inScheme nexus:ai-risk-ontology .

nexus:stakeholders a owl:ObjectProperty ;
    rdfs:label "stakeholders" ;
    skos:definition "A list of stakeholders" ;
    skos:inScheme nexus:ai-risk-ontology .

nexus:supported_languages a owl:DatatypeProperty ;
    rdfs:label "supported_languages" ;
    rdfs:range xsd:string ;
    skos:definition "A list of languages, expressed as ISO two letter codes. For example, 'jp, fr, en, de'" ;
    skos:inScheme nexus:ai_system .

nexus:taxonomies a owl:ObjectProperty ;
    rdfs:label "taxonomies" ;
    skos:definition "A list of AI risk taxonomies" ;
    skos:inScheme nexus:ai-risk-ontology .

nexus:terms a owl:ObjectProperty ;
    rdfs:label "terms" ;
    skos:definition "A list of terms from a vocabulary" ;
    skos:inScheme nexus:ai-risk-ontology .

nexus:vocabularies a owl:ObjectProperty ;
    rdfs:label "vocabularies" ;
    skos:definition "A list of vocabularies" ;
    skos:inScheme nexus:ai-risk-ontology .

nexus:Action a owl:Class ;
    rdfs:label "Action" ;
    rdfs:subClassOf [ a owl:Restriction ;
            owl:maxCardinality 1 ;
            owl:onProperty nexus:isDefinedByTaxonomy ],
        [ a owl:Restriction ;
            owl:minCardinality 0 ;
            owl:onProperty nexus:hasDocumentation ],
        [ a owl:Restriction ;
            owl:allValuesFrom xsd:string ;
            owl:onProperty nexus:hasAiActorTask ],
        [ a owl:Restriction ;
            owl:minCardinality 0 ;
            owl:onProperty nexus:hasRelatedRisk ],
        [ a owl:Restriction ;
            owl:minCardinality 0 ;
            owl:onProperty nexus:isDefinedByTaxonomy ],
        [ a owl:Restriction ;
            owl:allValuesFrom nexus:RiskTaxonomy ;
            owl:onProperty nexus:isDefinedByTaxonomy ],
        [ a owl:Restriction ;
            owl:allValuesFrom [ owl:intersectionOf ( [ owl:unionOf ( nexus:RiskConcept nexus:Term ) ] nexus:Risk ) ] ;
            owl:onProperty nexus:hasRelatedRisk ],
        [ a owl:Restriction ;
            owl:minCardinality 0 ;
            owl:onProperty nexus:hasAiActorTask ],
        [ a owl:Restriction ;
            owl:allValuesFrom nexus:Documentation ;
            owl:onProperty nexus:hasDocumentation ],
        nexus:Entity ;
    skos:definition "Action to remediate a risk" ;
    skos:inScheme nexus:ai_risk .

nexus:Adapter a owl:Class ;
    rdfs:label "Adapter" ;
    rdfs:subClassOf [ a owl:Restriction ;
            owl:allValuesFrom nexus:License ;
            owl:onProperty nexus:hasLicense ],
        [ a owl:Restriction ;
            owl:allValuesFrom nexus:AdapterType ;
            owl:onProperty nexus:hasAdapterType ],
        [ a owl:Restriction ;
            owl:allValuesFrom nexus:LargeLanguageModel ;
            owl:onProperty nexus:adaptsModel ],
        [ a owl:Restriction ;
            owl:allValuesFrom nexus:Vocabulary ;
            owl:onProperty nexus:isDefinedByVocabulary ],
        [ a owl:Restriction ;
            owl:minCardinality 0 ;
            owl:onProperty nexus:adaptsModel ],
        [ a owl:Restriction ;
            owl:maxCardinality 1 ;
            owl:onProperty nexus:adaptsModel ],
        [ a owl:Restriction ;
            owl:allValuesFrom [ owl:intersectionOf ( [ owl:unionOf ( nexus:RiskConcept nexus:Term ) ] nexus:Risk ) ] ;
            owl:onProperty nexus:hasRelatedRisk ],
        [ a owl:Restriction ;
            owl:minCardinality 0 ;
            owl:onProperty nexus:hasDocumentation ],
        [ a owl:Restriction ;
            owl:allValuesFrom nexus:Documentation ;
            owl:onProperty nexus:hasDocumentation ],
        [ a owl:Restriction ;
            owl:maxCardinality 1 ;
            owl:onProperty nexus:hasAdapterType ],
        [ a owl:Restriction ;
            owl:minCardinality 0 ;
            owl:onProperty nexus:hasRelatedRisk ],
        [ a owl:Restriction ;
            owl:minCardinality 0 ;
            owl:onProperty nexus:hasAdapterType ],
        [ a owl:Restriction ;
            owl:maxCardinality 1 ;
            owl:onProperty nexus:hasLicense ],
        [ a owl:Restriction ;
            owl:minCardinality 0 ;
            owl:onProperty nexus:isDefinedByVocabulary ],
        [ a owl:Restriction ;
            owl:maxCardinality 1 ;
            owl:onProperty nexus:isDefinedByVocabulary ],
        [ a owl:Restriction ;
            owl:minCardinality 0 ;
            owl:onProperty nexus:hasLicense ],
        nexus:Entity,
        nexus:LargeLanguageModel ;
    skos:definition "Adapter-based methods add extra trainable parameters after the attention and fully-connected layers of a frozen pretrained model to reduce memory-usage and speed up training. The adapters are typically small but demonstrate comparable performance to a fully finetuned model and enable training larger models with fewer resources. (https://huggingface.co/docs/peft/en/conceptual_guides/adapter)" ;
    skos:inScheme nexus:ai_intrinsic .

nexus:AiEvalResult a owl:Class ;
    rdfs:label "AiEvalResult" ;
    rdfs:subClassOf [ a owl:Restriction ;
            owl:allValuesFrom nexus:AiEval ;
            owl:onProperty nexus:isResultOf ],
        [ a owl:Restriction ;
            owl:maxCardinality 1 ;
            owl:onProperty nexus:isResultOf ],
        [ a owl:Restriction ;
            owl:minCardinality 0 ;
            owl:onProperty nexus:isResultOf ],
        nexus:Entity,
        nexus:Fact ;
    skos:definition "The result of an evaluation for a specific AI model." ;
    skos:exactMatch <https://www.w3.org/TR/vocab-dqv/QualityMeasurement> ;
    skos:inScheme nexus:ai_eval .

nexus:AiTask a owl:Class ;
    rdfs:label "AiTask" ;
    rdfs:subClassOf nexus:Entity ;
    skos:definition "A task, such as summarization and classification, performed by an AI." ;
    skos:exactMatch airo:AiCapability ;
    skos:inScheme nexus:ai_system .

nexus:BaseAi a owl:Class ;
    rdfs:label "BaseAi" ;
    rdfs:subClassOf [ a owl:Restriction ;
            owl:allValuesFrom nexus:AiTask ;
            owl:onProperty nexus:performsTask ],
        [ a owl:Restriction ;
            owl:minCardinality 0 ;
            owl:onProperty nexus:producer ],
        [ a owl:Restriction ;
            owl:minCardinality 0 ;
            owl:onProperty nexus:hasModelCard ],
        [ a owl:Restriction ;
            owl:maxCardinality 1 ;
            owl:onProperty nexus:isProvidedBy ],
        [ a owl:Restriction ;
            owl:minCardinality 0 ;
            owl:onProperty nexus:performsTask ],
        [ a owl:Restriction ;
            owl:maxCardinality 1 ;
            owl:onProperty nexus:producer ],
        [ a owl:Restriction ;
            owl:minCardinality 0 ;
            owl:onProperty nexus:hasLicense ],
        [ a owl:Restriction ;
            owl:minCardinality 0 ;
            owl:onProperty nexus:hasDocumentation ],
        [ a owl:Restriction ;
            owl:allValuesFrom xsd:string ;
            owl:onProperty nexus:hasModelCard ],
        [ a owl:Restriction ;
            owl:minCardinality 0 ;
            owl:onProperty nexus:isProvidedBy ],
        [ a owl:Restriction ;
            owl:allValuesFrom nexus:License ;
            owl:onProperty nexus:hasLicense ],
        [ a owl:Restriction ;
            owl:maxCardinality 1 ;
            owl:onProperty nexus:hasLicense ],
        [ a owl:Restriction ;
            owl:allValuesFrom nexus:Organization ;
            owl:onProperty nexus:producer ],
        [ a owl:Restriction ;
            owl:allValuesFrom nexus:AiProvider ;
            owl:onProperty nexus:isProvidedBy ],
        [ a owl:Restriction ;
            owl:allValuesFrom nexus:Documentation ;
            owl:onProperty nexus:hasDocumentation ],
        nexus:Entity ;
    skos:definition "Any type of AI, be it a LLM, RL agent, SVM, etc." ;
    skos:inScheme nexus:ai_system .

nexus:adaptsModel a owl:ObjectProperty ;
    rdfs:label "adaptsModel" ;
    rdfs:range nexus:LargeLanguageModel ;
    skos:definition "The LargeLanguageModel being adapted" ;
    skos:inScheme nexus:ai_intrinsic .

nexus:architecture a owl:DatatypeProperty ;
    rdfs:label "architecture" ;
    rdfs:range xsd:string ;
    skos:definition "A description of the architecture of an AI such as 'Decoder-only'." ;
    skos:inScheme nexus:ai_system .

nexus:bestValue a owl:DatatypeProperty ;
    rdfs:label "bestValue" ;
    skos:definition "Annotation of the best possible result of the evaluation" ;
    skos:inScheme nexus:ai_eval .

nexus:carbon_emitted a owl:DatatypeProperty ;
    rdfs:label "carbon_emitted" ;
    rdfs:range [ a rdfs:Datatype ;
            owl:intersectionOf ( xsd:float [ a rdfs:Datatype ;
                        owl:onDatatype xsd:integer ;
                        owl:withRestrictions ( [ xsd:minInclusive 0 ] ) ] ) ] ;
    skos:definition "The number of tons of carbon dioxide equivalent that are emitted during training" ;
    skos:inScheme nexus:energy .

nexus:concern a owl:DatatypeProperty ;
    rdfs:label "concern" ;
    skos:definition "Some explanation about the concern related to an AI risk" ;
    skos:inScheme nexus:ai_risk .

nexus:contextWindowSize a owl:DatatypeProperty ;
    rdfs:label "contextWindowSize" ;
    rdfs:range [ a rdfs:Datatype ;
            owl:intersectionOf ( xsd:integer [ a rdfs:Datatype ;
                        owl:onDatatype xsd:integer ;
                        owl:withRestrictions ( [ xsd:minInclusive 0 ] ) ] ) ] ;
    skos:definition "The total length, in bytes, of an AI model's context window." ;
    skos:inScheme nexus:ai_system .

nexus:dateCreated a owl:DatatypeProperty ;
    rdfs:label "dateCreated" ;
    rdfs:range xsd:date ;
    skos:definition "The date on which the entity was created." ;
    skos:inScheme nexus:common .

nexus:dateModified a owl:DatatypeProperty ;
    rdfs:label "dateModified" ;
    rdfs:range xsd:date ;
    skos:definition "The date on which the entity was most recently modified." ;
    skos:inScheme nexus:common .

nexus:describesAiEval a owl:ObjectProperty ;
    rdfs:label "describesAiEval" ;
    rdfs:domain nexus:BenchmarkMetadataCard ;
    rdfs:range nexus:AiEval ;
    owl:inverseOf nexus:hasBenchmarkMetadata ;
    skos:definition "A relationship where a BenchmarkMetadataCard describes and AI evaluation (benchmark)." ;
    skos:inScheme nexus:ai_eval .

nexus:description a owl:DatatypeProperty ;
    rdfs:label "description" ;
    skos:definition "The description of an entity" ;
    skos:inScheme nexus:common .

nexus:descriptor a owl:DatatypeProperty ;
    rdfs:label "descriptor" ;
    skos:definition "Annotates whether an AI risk is a traditional risk, specific to or amplified by AI." ;
    skos:inScheme nexus:ai_risk .

nexus:evidence a owl:DatatypeProperty ;
    rdfs:label "evidence" ;
    skos:definition "Evidence provides a source (typical a chunk, paragraph or link) describing where some value was found or how it was generated." ;
    skos:inScheme nexus:common .

nexus:fine_tuning a owl:DatatypeProperty ;
    rdfs:label "fine_tuning" ;
    rdfs:range xsd:string ;
    skos:definition "A description of the fine-tuning mechanism(s) applied to a model." ;
    skos:inScheme nexus:ai_system .

nexus:gpu_hours a owl:DatatypeProperty ;
    rdfs:label "gpu_hours" ;
    rdfs:range [ a rdfs:Datatype ;
            owl:intersectionOf ( xsd:integer [ a rdfs:Datatype ;
                        owl:onDatatype xsd:integer ;
                        owl:withRestrictions ( [ xsd:minInclusive 0 ] ) ] ) ] ;
    skos:definition "GPU consumption in terms of hours" ;
    skos:inScheme nexus:energy .

nexus:grants_license a owl:ObjectProperty ;
    rdfs:label "grants_license" ;
    rdfs:range nexus:License ;
    skos:definition "A relationship from a granting entity such as an Organization to a License instance." ;
    skos:inScheme nexus:common .

nexus:hasAdapterType a owl:ObjectProperty ;
    rdfs:label "hasAdapterType" ;
    rdfs:range nexus:AdapterType ;
    skos:definition "The Adapter type, for example: LORA, ALORA, X-LORA" ;
    skos:inScheme nexus:ai_intrinsic .

nexus:hasAnnotation a owl:DatatypeProperty ;
    rdfs:label "hasAnnotation" ;
    skos:definition "The process used to annotate or label the dataset, including who or what performed the annotations (e.g., human annotators, automated processes)." ;
    skos:inScheme nexus:ai_eval .

nexus:hasAudience a owl:DatatypeProperty ;
    rdfs:label "hasAudience" ;
    skos:definition "The intended audience, such as researchers, developers, policymakers, etc." ;
    skos:inScheme nexus:ai_eval .

nexus:hasBaselineResults a owl:DatatypeProperty ;
    rdfs:label "hasBaselineResults" ;
    skos:definition "The results of well-known or widely used models to give context to new performance scores." ;
    skos:inScheme nexus:ai_eval .

nexus:hasBenchmarkMetadata a owl:ObjectProperty ;
    rdfs:label "hasBenchmarkMetadata" ;
    rdfs:domain nexus:AiEval ;
    rdfs:range nexus:BenchmarkMetadataCard ;
    owl:inverseOf nexus:describesAiEval ;
    skos:definition "A relationship to a Benchmark Metadata Card which contains metadata about the benchmark." ;
    skos:inScheme nexus:ai_eval .

nexus:hasConsequence a owl:ObjectProperty ;
    rdfs:label "hasConsequence" ;
    rdfs:domain nexus:RiskConcept ;
    rdfs:range nexus:Consequence ;
    skos:definition "Indicates consequence(s) possible or arising from specified concept" ;
    skos:inScheme nexus:ai_risk .

nexus:hasConsiderationComplianceWithRegulations a owl:DatatypeProperty ;
    rdfs:label "hasConsiderationComplianceWithRegulations" ;
    skos:definition "Compliance with relevant legal or ethical regulations (if applicable)." ;
    skos:inScheme nexus:ai_eval .

nexus:hasConsiderationConsentProcedures a owl:DatatypeProperty ;
    rdfs:label "hasConsiderationConsentProcedures" ;
    skos:definition "Information on how consent was obtained (if applicable), especially for datasets involving personal data." ;
    skos:inScheme nexus:ai_eval .

nexus:hasConsiderationPrivacyAndAnonymity a owl:DatatypeProperty ;
    rdfs:label "hasConsiderationPrivacyAndAnonymity" ;
    skos:definition "How any personal or sensitive data is handled and whether any anonymization techniques are applied." ;
    skos:inScheme nexus:ai_eval .

nexus:hasDataFormat a owl:DatatypeProperty ;
    rdfs:label "hasDataFormat" ;
    skos:definition "The structure and modality of the data (e.g., sentence pairs, question-answer format, tabular data)." ;
    skos:inScheme nexus:ai_eval .

nexus:hasDataSize a owl:DatatypeProperty ;
    rdfs:label "hasDataSize" ;
    skos:definition "The size of the dataset, including the number of data points or examples." ;
    skos:inScheme nexus:ai_eval .

nexus:hasDemographicAnalysis a owl:DatatypeProperty ;
    rdfs:label "hasDemographicAnalysis" ;
    skos:definition "How the benchmark evaluates performance across different demographic groups (e.g., gender, race)." ;
    skos:inScheme nexus:ai_eval .

nexus:hasEuAiSystemType a owl:ObjectProperty ;
    rdfs:label "hasEuAiSystemType" ;
    rdfs:range nexus:AiSystemType ;
    skos:definition "The type of system as defined by the EU AI Act." ;
    skos:inScheme nexus:eu_ai_act .

nexus:hasEuRiskCategory a owl:ObjectProperty ;
    rdfs:label "hasEuRiskCategory" ;
    rdfs:range nexus:EuAiRiskCategory ;
    skos:definition "The risk category of an AI system as defined by the EU AI Act." ;
    skos:inScheme nexus:eu_ai_act .

nexus:hasGoal a owl:DatatypeProperty ;
    rdfs:label "hasGoal" ;
    skos:definition "The specific goal or primary use case the benchmark is designed for." ;
    skos:inScheme nexus:ai_eval .

nexus:hasImpact a owl:ObjectProperty ;
    rdfs:label "hasImpact" ;
    rdfs:domain nexus:RiskConcept ;
    rdfs:range nexus:Impact ;
    skos:broadMatch <https://w3id.org/dpv#hasConsequence> ;
    skos:definition "Indicates impact(s) possible or arising as consequences from specified concept" ;
    skos:inScheme nexus:ai_risk .

nexus:hasImpactOn a owl:ObjectProperty ;
    rdfs:label "hasImpactOn" ;
    rdfs:domain nexus:RiskConcept ;
    rdfs:range nexus:Impact ;
    skos:broadMatch <https://w3id.org/dpv#hasConsequenceOn> ;
    skos:definition "Indicates impact(s) possible or arising as consequences from specified concept" ;
    skos:inScheme nexus:ai_risk .

nexus:hasLikelihood a owl:ObjectProperty ;
    rdfs:label "hasLikelihood" ;
    rdfs:domain nexus:RiskConcept ;
    rdfs:range nexus:Likelihood ;
    skos:definition "The likelihood or probability or chance of something taking place or occuring" ;
    skos:inScheme nexus:ai_risk .

nexus:hasSeverity a owl:ObjectProperty ;
    rdfs:label "hasSeverity" ;
    rdfs:domain nexus:RiskConcept ;
    rdfs:range nexus:Severity ;
    skos:definition "Indicates the severity associated with a concept" ;
    skos:inScheme nexus:ai_risk .

nexus:hasStatus a owl:ObjectProperty ;
    rdfs:label "hasStatus" ;
    rdfs:domain nexus:RiskConcept ;
    rdfs:range nexus:IncidentStatus ;
    skos:definition "Indicates the status of specified concept" ;
    skos:inScheme nexus:ai_risk .

nexus:hasVariant a owl:ObjectProperty ;
    rdfs:label "hasVariant" ;
    rdfs:domain nexus:RiskIncident ;
    rdfs:range nexus:RiskIncident ;
    skos:definition "Indicates an incident that shares the same causative factors, produces similar harms, and involves the same intelligent systems as a known AI incident." ;
    skos:inScheme nexus:ai_risk .

nexus:id a owl:DatatypeProperty ;
    rdfs:label "id" ;
    skos:definition "A unique identifier to this instance of the model element. Example identifiers include UUID, URI, URN, etc." ;
    skos:inScheme nexus:common .

nexus:isDetectedBy a owl:ObjectProperty ;
    rdfs:label "isDetectedBy" ;
    rdfs:domain nexus:RiskConcept ;
    rdfs:range nexus:RiskControl ;
    owl:inverseOf nexus:detectsRiskConcept ;
    skos:definition "A relationship where a risk, risk source, consequence, or impact is detected by a risk control." ;
    skos:inScheme nexus:ai_risk .

nexus:isResultOf a owl:ObjectProperty ;
    rdfs:label "isResultOf" ;
    rdfs:range nexus:AiEval ;
    skos:definition "A relationship indicating that an entity is the result of an AI evaluation." ;
    skos:inScheme nexus:ai_eval .

nexus:numParameters a owl:DatatypeProperty ;
    rdfs:label "numParameters" ;
    rdfs:range [ a rdfs:Datatype ;
            owl:intersectionOf ( xsd:integer [ a rdfs:Datatype ;
                        owl:onDatatype xsd:integer ;
                        owl:withRestrictions ( [ xsd:minInclusive 0 ] ) ] ) ] ;
    skos:definition "A property indicating the number of parameters in a LLM." ;
    skos:inScheme nexus:ai_system .

nexus:numTrainingTokens a owl:DatatypeProperty ;
    rdfs:label "numTrainingTokens" ;
    rdfs:range [ a rdfs:Datatype ;
            owl:intersectionOf ( xsd:integer [ a rdfs:Datatype ;
                        owl:onDatatype xsd:integer ;
                        owl:withRestrictions ( [ xsd:minInclusive 0 ] ) ] ) ] ;
    skos:definition "The number of tokens a AI model was trained on." ;
    skos:inScheme nexus:ai_system .

nexus:overview a owl:DatatypeProperty ;
    rdfs:label "overview" ;
    skos:definition "A brief description of the benchmark's main goals and scope." ;
    skos:inScheme nexus:ai_eval .

nexus:phase a owl:DatatypeProperty ;
    rdfs:label "phase" ;
    skos:definition "Annotation whether an AI risk shows specifically during the training-tuning or inference phase." ;
    skos:inScheme nexus:ai_risk .

nexus:power_consumption_w a owl:DatatypeProperty ;
    rdfs:label "power_consumption_w" ;
    rdfs:range [ a rdfs:Datatype ;
            owl:intersectionOf ( xsd:integer [ a rdfs:Datatype ;
                        owl:onDatatype xsd:integer ;
                        owl:withRestrictions ( [ xsd:minInclusive 0 ] ) ] ) ] ;
    skos:definition "power consumption in Watts" ;
    skos:inScheme nexus:energy .

nexus:producer a owl:ObjectProperty ;
    rdfs:label "producer" ;
    rdfs:range nexus:Organization ;
    skos:definition "A relationship to the Organization instance which produces this instance." ;
    skos:inScheme nexus:common .

nexus:provider a owl:ObjectProperty ;
    rdfs:label "provider" ;
    rdfs:range nexus:Organization ;
    skos:definition "A relationship to the Organization instance that provides this instance." ;
    skos:inScheme nexus:common .

nexus:source_uri a owl:DatatypeProperty ;
    rdfs:label "source_uri" ;
    skos:definition "The uri of the incident" ;
    skos:inScheme nexus:ai_risk .

nexus:tag a owl:DatatypeProperty ;
    rdfs:label "tag" ;
    skos:definition "A shost version of the name" ;
    skos:inScheme nexus:ai_risk .

nexus:text a owl:DatatypeProperty ;
    rdfs:label "text" ;
    skos:definition "The question itself" ;
    skos:inScheme nexus:ai_eval .

nexus:type a owl:DatatypeProperty ;
    rdfs:label "type" ;
    skos:definition "Annotation whether an AI risk occurs at input or output or is non-technical." ;
    skos:inScheme nexus:ai_risk .

nexus:url a owl:DatatypeProperty ;
    rdfs:label "url" ;
    rdfs:range xsd:anyURI ;
    skos:definition "An optional URL associated with this instance." ;
    skos:inScheme nexus:common .

nexus:value a owl:DatatypeProperty ;
    rdfs:label "value" ;
    skos:definition "Some numeric or string value" ;
    skos:inScheme nexus:common .

nexus:BenchmarkMetadataCard a owl:Class ;
    rdfs:label "BenchmarkMetadataCard" ;
    rdfs:subClassOf [ a owl:Restriction ;
            owl:allValuesFrom nexus:Documentation ;
            owl:onProperty nexus:hasDocumentation ],
        [ a owl:Restriction ;
            owl:minCardinality 0 ;
            owl:onProperty nexus:hasDataSize ],
        [ a owl:Restriction ;
            owl:allValuesFrom xsd:string ;
            owl:onProperty nexus:hasAnnotation ],
        [ a owl:Restriction ;
            owl:minCardinality 0 ;
            owl:onProperty nexus:hasDataFormat ],
        [ a owl:Restriction ;
            owl:maxCardinality 1 ;
            owl:onProperty nexus:hasGoal ],
        [ a owl:Restriction ;
            owl:allValuesFrom xsd:string ;
            owl:onProperty nexus:hasAudience ],
        [ a owl:Restriction ;
            owl:allValuesFrom xsd:string ;
            owl:onProperty nexus:hasConsiderationComplianceWithRegulations ],
        [ a owl:Restriction ;
            owl:allValuesFrom xsd:string ;
            owl:onProperty nexus:name ],
        [ a owl:Restriction ;
            owl:allValuesFrom xsd:string ;
            owl:onProperty nexus:hasGoal ],
        [ a owl:Restriction ;
            owl:minCardinality 0 ;
            owl:onProperty nexus:hasMetrics ],
        [ a owl:Restriction ;
            owl:allValuesFrom xsd:string ;
            owl:onProperty nexus:hasMethods ],
        [ a owl:Restriction ;
            owl:allValuesFrom xsd:string ;
            owl:onProperty nexus:hasResources ],
        [ a owl:Restriction ;
            owl:allValuesFrom xsd:string ;
            owl:onProperty nexus:hasMetrics ],
        [ a owl:Restriction ;
            owl:minCardinality 0 ;
            owl:onProperty nexus:hasLimitations ],
        [ a owl:Restriction ;
            owl:minCardinality 0 ;
            owl:onProperty nexus:overview ],
        [ a owl:Restriction ;
            owl:minCardinality 0 ;
            owl:onProperty nexus:describesAiEval ],
        [ a owl:Restriction ;
            owl:minCardinality 0 ;
            owl:onProperty nexus:hasResources ],
        [ a owl:Restriction ;
            owl:allValuesFrom xsd:string ;
            owl:onProperty nexus:hasDataFormat ],
        [ a owl:Restriction ;
            owl:minCardinality 0 ;
            owl:onProperty nexus:hasRelatedRisk ],
        [ a owl:Restriction ;
            owl:maxCardinality 1 ;
            owl:onProperty nexus:hasBaselineResults ],
        [ a owl:Restriction ;
            owl:allValuesFrom xsd:string ;
            owl:onProperty nexus:hasDataSource ],
        [ a owl:Restriction ;
            owl:allValuesFrom nexus:AiEval ;
            owl:onProperty nexus:describesAiEval ],
        [ a owl:Restriction ;
            owl:minCardinality 0 ;
            owl:onProperty nexus:hasValidation ],
        [ a owl:Restriction ;
            owl:maxCardinality 1 ;
            owl:onProperty nexus:hasConsiderationComplianceWithRegulations ],
        [ a owl:Restriction ;
            owl:maxCardinality 1 ;
            owl:onProperty nexus:overview ],
        [ a owl:Restriction ;
            owl:allValuesFrom xsd:string ;
            owl:onProperty nexus:hasBaselineResults ],
        [ a owl:Restriction ;
            owl:allValuesFrom xsd:string ;
            owl:onProperty nexus:hasConsiderationConsentProcedures ],
        [ a owl:Restriction ;
            owl:minCardinality 0 ;
            owl:onProperty nexus:hasLanguages ],
        [ a owl:Restriction ;
            owl:minCardinality 0 ;
            owl:onProperty nexus:hasDemographicAnalysis ],
        [ a owl:Restriction ;
            owl:minCardinality 0 ;
            owl:onProperty nexus:hasConsiderationPrivacyAndAnonymity ],
        [ a owl:Restriction ;
            owl:minCardinality 0 ;
            owl:onProperty nexus:hasOutOfScopeUses ],
        [ a owl:Restriction ;
            owl:allValuesFrom xsd:string ;
            owl:onProperty nexus:hasDataSize ],
        [ a owl:Restriction ;
            owl:minCardinality 0 ;
            owl:onProperty nexus:hasDocumentation ],
        [ a owl:Restriction ;
            owl:allValuesFrom xsd:string ;
            owl:onProperty nexus:hasOutOfScopeUses ],
        [ a owl:Restriction ;
            owl:maxCardinality 1 ;
            owl:onProperty nexus:hasDataSize ],
        [ a owl:Restriction ;
            owl:minCardinality 0 ;
            owl:onProperty nexus:name ],
        [ a owl:Restriction ;
            owl:minCardinality 0 ;
            owl:onProperty nexus:hasTasks ],
        [ a owl:Restriction ;
            owl:minCardinality 0 ;
            owl:onProperty nexus:hasDomains ],
        [ a owl:Restriction ;
            owl:minCardinality 0 ;
            owl:onProperty nexus:hasInterpretation ],
        [ a owl:Restriction ;
            owl:minCardinality 0 ;
            owl:onProperty nexus:hasBaselineResults ],
        [ a owl:Restriction ;
            owl:minCardinality 0 ;
            owl:onProperty nexus:hasMethods ],
        [ a owl:Restriction ;
            owl:minCardinality 0 ;
            owl:onProperty nexus:hasLicense ],
        [ a owl:Restriction ;
            owl:allValuesFrom xsd:string ;
            owl:onProperty nexus:hasDataType ],
        [ a owl:Restriction ;
            owl:allValuesFrom xsd:string ;
            owl:onProperty nexus:hasLimitations ],
        [ a owl:Restriction ;
            owl:allValuesFrom xsd:string ;
            owl:onProperty nexus:hasCalculation ],
        [ a owl:Restriction ;
            owl:minCardinality 0 ;
            owl:onProperty nexus:hasAudience ],
        [ a owl:Restriction ;
            owl:maxCardinality 1 ;
            owl:onProperty nexus:hasConsiderationConsentProcedures ],
        [ a owl:Restriction ;
            owl:maxCardinality 1 ;
            owl:onProperty nexus:hasDemographicAnalysis ],
        [ a owl:Restriction ;
            owl:allValuesFrom xsd:string ;
            owl:onProperty nexus:hasDemographicAnalysis ],
        [ a owl:Restriction ;
            owl:allValuesFrom xsd:string ;
            owl:onProperty nexus:hasConsiderationPrivacyAndAnonymity ],
        [ a owl:Restriction ;
            owl:minCardinality 0 ;
            owl:onProperty nexus:hasConsiderationConsentProcedures ],
        [ a owl:Restriction ;
            owl:maxCardinality 1 ;
            owl:onProperty nexus:hasAudience ],
        [ a owl:Restriction ;
            owl:minCardinality 0 ;
            owl:onProperty nexus:hasAnnotation ],
        [ a owl:Restriction ;
            owl:allValuesFrom nexus:License ;
            owl:onProperty nexus:hasLicense ],
        [ a owl:Restriction ;
            owl:allValuesFrom xsd:string ;
            owl:onProperty nexus:hasSimilarBenchmarks ],
        [ a owl:Restriction ;
            owl:maxCardinality 1 ;
            owl:onProperty nexus:name ],
        [ a owl:Restriction ;
            owl:maxCardinality 1 ;
            owl:onProperty nexus:hasConsiderationPrivacyAndAnonymity ],
        [ a owl:Restriction ;
            owl:maxCardinality 1 ;
            owl:onProperty nexus:hasLicense ],
        [ a owl:Restriction ;
            owl:maxCardinality 1 ;
            owl:onProperty nexus:hasDataFormat ],
        [ a owl:Restriction ;
            owl:minCardinality 0 ;
            owl:onProperty nexus:hasConsiderationComplianceWithRegulations ],
        [ a owl:Restriction ;
            owl:allValuesFrom xsd:string ;
            owl:onProperty nexus:hasLanguages ],
        [ a owl:Restriction ;
            owl:allValuesFrom xsd:string ;
            owl:onProperty nexus:hasTasks ],
        [ a owl:Restriction ;
            owl:allValuesFrom xsd:string ;
            owl:onProperty nexus:hasDomains ],
        [ a owl:Restriction ;
            owl:minCardinality 0 ;
            owl:onProperty nexus:hasSimilarBenchmarks ],
        [ a owl:Restriction ;
            owl:minCardinality 0 ;
            owl:onProperty nexus:hasDataType ],
        [ a owl:Restriction ;
            owl:allValuesFrom [ owl:intersectionOf ( [ owl:unionOf ( nexus:RiskConcept nexus:Term ) ] nexus:Risk ) ] ;
            owl:onProperty nexus:hasRelatedRisk ],
        [ a owl:Restriction ;
            owl:minCardinality 0 ;
            owl:onProperty nexus:hasGoal ],
        [ a owl:Restriction ;
            owl:allValuesFrom xsd:string ;
            owl:onProperty nexus:overview ],
        [ a owl:Restriction ;
            owl:allValuesFrom xsd:string ;
            owl:onProperty nexus:hasValidation ],
        [ a owl:Restriction ;
            owl:maxCardinality 1 ;
            owl:onProperty nexus:hasAnnotation ],
        [ a owl:Restriction ;
            owl:allValuesFrom xsd:string ;
            owl:onProperty nexus:hasInterpretation ],
        [ a owl:Restriction ;
            owl:minCardinality 0 ;
            owl:onProperty nexus:hasCalculation ],
        [ a owl:Restriction ;
            owl:minCardinality 0 ;
            owl:onProperty nexus:hasDataSource ],
        nexus:Entity ;
    skos:definition "Benchmark metadata cards offer a standardized way to document LLM benchmarks clearly and transparently. Inspired by Model Cards and Datasheets, Benchmark metadata cards help researchers and practitioners understand exactly what benchmarks test, how they relate to real-world risks, and how to interpret their results responsibly.  This is an implementation of the design set out in 'BenchmarkCards: Large Language Model and Risk Reporting' (https://doi.org/10.48550/arXiv.2410.12974)" ;
    skos:exactMatch nexus:benchmarkmetadatacard ;
    skos:inScheme nexus:ai_eval .

nexus:Impact a owl:Class ;
    rdfs:label "Impact" ;
    rdfs:subClassOf nexus:Entity,
        nexus:RiskConcept ;
    skos:exactMatch <https://w3id.org/dpv#Impact> ;
    skos:inScheme nexus:ai_risk .

nexus:LargeLanguageModel a owl:Class ;
    rdfs:label "LargeLanguageModel" ;
    rdfs:subClassOf [ a owl:Restriction ;
            owl:allValuesFrom nexus:Modality ;
            owl:onProperty nexus:hasInputModality ],
        [ a owl:Restriction ;
            owl:maxCardinality 1 ;
            owl:onProperty nexus:isPartOf ],
        [ a owl:Restriction ;
            owl:minCardinality 0 ;
            owl:onProperty nexus:hasInputModality ],
        [ a owl:Restriction ;
            owl:allValuesFrom [ a rdfs:Datatype ;
                    owl:intersectionOf ( xsd:integer [ a rdfs:Datatype ;
                                owl:onDatatype xsd:integer ;
                                owl:withRestrictions ( [ xsd:minInclusive 0 ] ) ] ) ] ;
            owl:onProperty nexus:numTrainingTokens ],
        [ a owl:Restriction ;
            owl:allValuesFrom nexus:Dataset ;
            owl:onProperty nexus:hasTrainingData ],
        [ a owl:Restriction ;
            owl:maxCardinality 1 ;
            owl:onProperty nexus:numTrainingTokens ],
        [ a owl:Restriction ;
            owl:allValuesFrom nexus:LargeLanguageModelFamily ;
            owl:onProperty nexus:isPartOf ],
        [ a owl:Restriction ;
            owl:minCardinality 0 ;
            owl:onProperty nexus:hasOutputModality ],
        [ a owl:Restriction ;
            owl:allValuesFrom xsd:string ;
            owl:onProperty nexus:supported_languages ],
        [ a owl:Restriction ;
            owl:maxCardinality 1 ;
            owl:onProperty nexus:numParameters ],
        [ a owl:Restriction ;
            owl:minCardinality 0 ;
            owl:onProperty nexus:fine_tuning ],
        [ a owl:Restriction ;
            owl:allValuesFrom [ a rdfs:Datatype ;
                    owl:intersectionOf ( xsd:integer [ a rdfs:Datatype ;
                                owl:onDatatype xsd:integer ;
                                owl:withRestrictions ( [ xsd:minInclusive 0 ] ) ] ) ] ;
            owl:onProperty nexus:contextWindowSize ],
        [ a owl:Restriction ;
            owl:maxCardinality 1 ;
            owl:onProperty nexus:contextWindowSize ],
        [ a owl:Restriction ;
            owl:allValuesFrom xsd:string ;
            owl:onProperty nexus:fine_tuning ],
        [ a owl:Restriction ;
            owl:minCardinality 0 ;
            owl:onProperty nexus:contextWindowSize ],
        [ a owl:Restriction ;
            owl:minCardinality 0 ;
            owl:onProperty nexus:isPartOf ],
        [ a owl:Restriction ;
            owl:allValuesFrom [ a rdfs:Datatype ;
                    owl:intersectionOf ( xsd:integer [ a rdfs:Datatype ;
                                owl:onDatatype xsd:integer ;
                                owl:withRestrictions ( [ xsd:minInclusive 0 ] ) ] ) ] ;
            owl:onProperty nexus:numParameters ],
        [ a owl:Restriction ;
            owl:minCardinality 0 ;
            owl:onProperty nexus:supported_languages ],
        [ a owl:Restriction ;
            owl:minCardinality 0 ;
            owl:onProperty nexus:numTrainingTokens ],
        [ a owl:Restriction ;
            owl:minCardinality 0 ;
            owl:onProperty nexus:hasTrainingData ],
        [ a owl:Restriction ;
            owl:minCardinality 0 ;
            owl:onProperty nexus:numParameters ],
        [ a owl:Restriction ;
            owl:maxCardinality 1 ;
            owl:onProperty nexus:fine_tuning ],
        [ a owl:Restriction ;
            owl:allValuesFrom nexus:Modality ;
            owl:onProperty nexus:hasOutputModality ],
        nexus:AiModel ;
    skos:altLabel "LLM" ;
    skos:definition "A large language model (LLM) is an AI model which supports a range of language-related tasks such as generation, summarization, classification, among others. A LLM is implemented as an artificial neural networks using a transformer architecture." ;
    skos:inScheme nexus:ai_system .

nexus:broadMatch a owl:ObjectProperty ;
    rdfs:label "broadMatch" ;
    rdfs:range [ owl:intersectionOf ( [ owl:unionOf ( nexus:Risk nexus:RiskGroup ) ] nexus:Any ) ] ;
    skos:definition "The property is used to state a hierarchical mapping link between two concepts, indicating that the concept linked to, is a broader concept than the originating concept." ;
    skos:inScheme nexus:ai_risk .

nexus:closeMatch a owl:ObjectProperty ;
    rdfs:label "closeMatch" ;
    rdfs:range [ owl:intersectionOf ( [ owl:unionOf ( nexus:Risk nexus:RiskGroup ) ] nexus:Any ) ] ;
    skos:definition "The property is used to link two concepts that are sufficiently similar that they can be used interchangeably in some information retrieval applications." ;
    skos:inScheme nexus:ai_risk .

nexus:exactMatch a owl:ObjectProperty ;
    rdfs:label "exactMatch" ;
    rdfs:range [ owl:intersectionOf ( [ owl:unionOf ( nexus:Risk nexus:RiskGroup ) ] nexus:Any ) ] ;
    skos:definition "The property is used to link two concepts, indicating a high degree of confidence that the concepts can be used interchangeably across a wide range of information retrieval applications" ;
    skos:inScheme nexus:ai_risk .

nexus:hasTasks a owl:DatatypeProperty ;
    rdfs:label "hasTasks" ;
    skos:definition "The tasks or evaluations the benchmark is intended to assess." ;
    skos:inScheme nexus:ai_eval .

nexus:isComposedOf a owl:DatatypeProperty ;
    rdfs:label "isComposedOf" ;
    skos:definition "Relationship indicating the some entity is composed of other entities (including some of the same type)." ;
    skos:inScheme nexus:common .

nexus:narrowMatch a owl:ObjectProperty ;
    rdfs:label "narrowMatch" ;
    rdfs:range [ owl:intersectionOf ( [ owl:unionOf ( nexus:Risk nexus:RiskGroup ) ] nexus:Any ) ] ;
    skos:definition "The property is used to state a hierarchical mapping link between two concepts, indicating that the concept linked to, is a narrower concept than the originating concept." ;
    skos:inScheme nexus:ai_risk .

nexus:relatedMatch a owl:ObjectProperty ;
    rdfs:label "relatedMatch" ;
    rdfs:range [ owl:intersectionOf ( [ owl:unionOf ( nexus:Risk nexus:RiskGroup ) ] nexus:Any ) ] ;
    skos:definition "The property skos:relatedMatch is used to state an associative mapping link between two concepts." ;
    skos:inScheme nexus:ai_risk .

nexus:AdapterType a owl:Class ;
    owl:unionOf ( <https://ibm.github.io/risk-atlas-nexus/ontology/AdapterType#LORA> <https://ibm.github.io/risk-atlas-nexus/ontology/AdapterType#ALORA> <https://ibm.github.io/risk-atlas-nexus/ontology/AdapterType#X-LORA> ) ;
    linkml:permissible_values <https://ibm.github.io/risk-atlas-nexus/ontology/AdapterType#ALORA>,
        <https://ibm.github.io/risk-atlas-nexus/ontology/AdapterType#LORA>,
        <https://ibm.github.io/risk-atlas-nexus/ontology/AdapterType#X-LORA> .

nexus:Dataset a owl:Class ;
    rdfs:label "Dataset" ;
    rdfs:subClassOf [ a owl:Restriction ;
            owl:allValuesFrom nexus:License ;
            owl:onProperty nexus:hasLicense ],
        [ a owl:Restriction ;
            owl:maxCardinality 1 ;
            owl:onProperty nexus:hasLicense ],
        [ a owl:Restriction ;
            owl:minCardinality 0 ;
            owl:onProperty nexus:provider ],
        [ a owl:Restriction ;
            owl:maxCardinality 1 ;
            owl:onProperty nexus:provider ],
        [ a owl:Restriction ;
            owl:minCardinality 0 ;
            owl:onProperty nexus:hasLicense ],
        [ a owl:Restriction ;
            owl:allValuesFrom nexus:Organization ;
            owl:onProperty nexus:provider ],
        [ a owl:Restriction ;
            owl:allValuesFrom nexus:Documentation ;
            owl:onProperty nexus:hasDocumentation ],
        [ a owl:Restriction ;
            owl:minCardinality 0 ;
            owl:onProperty nexus:hasDocumentation ],
        nexus:Entity ;
    skos:definition "A body of structured information describing some topic(s) of interest." ;
    skos:exactMatch <http://schema.org/Dataset> ;
    skos:inScheme nexus:common .

nexus:Modality a owl:Class ;
    rdfs:label "Modality" ;
    rdfs:subClassOf nexus:Entity ;
    skos:definition "A modality supported by an Ai component. Examples include text, image, video." ;
    skos:exactMatch airo:Modality ;
    skos:inScheme nexus:ai_system .

nexus:RiskIncident a owl:Class ;
    rdfs:label "RiskIncident" ;
    rdfs:subClassOf [ a owl:Restriction ;
            owl:minCardinality 0 ;
            owl:onProperty nexus:hasLikelihood ],
        [ a owl:Restriction ;
            owl:maxCardinality 1 ;
            owl:onProperty nexus:hasVariant ],
        [ a owl:Restriction ;
            owl:minCardinality 0 ;
            owl:onProperty nexus:source_uri ],
        [ a owl:Restriction ;
            owl:minCardinality 0 ;
            owl:onProperty nexus:hasImpact ],
        [ a owl:Restriction ;
            owl:allValuesFrom nexus:Likelihood ;
            owl:onProperty nexus:hasLikelihood ],
        [ a owl:Restriction ;
            owl:maxCardinality 1 ;
            owl:onProperty nexus:hasConsequence ],
        [ a owl:Restriction ;
            owl:minCardinality 0 ;
            owl:onProperty nexus:hasConsequence ],
        [ a owl:Restriction ;
            owl:maxCardinality 1 ;
            owl:onProperty nexus:isDefinedByTaxonomy ],
        [ a owl:Restriction ;
            owl:minCardinality 0 ;
            owl:onProperty nexus:isDefinedByTaxonomy ],
        [ a owl:Restriction ;
            owl:allValuesFrom xsd:string ;
            owl:onProperty nexus:author ],
        [ a owl:Restriction ;
            owl:minCardinality 0 ;
            owl:onProperty nexus:author ],
        [ a owl:Restriction ;
            owl:maxCardinality 1 ;
            owl:onProperty nexus:hasLikelihood ],
        [ a owl:Restriction ;
            owl:allValuesFrom nexus:RiskTaxonomy ;
            owl:onProperty nexus:isDefinedByTaxonomy ],
        [ a owl:Restriction ;
            owl:maxCardinality 1 ;
            owl:onProperty nexus:hasStatus ],
        [ a owl:Restriction ;
            owl:allValuesFrom nexus:Severity ;
            owl:onProperty nexus:hasSeverity ],
        [ a owl:Restriction ;
            owl:allValuesFrom nexus:Impact ;
            owl:onProperty nexus:hasImpactOn ],
        [ a owl:Restriction ;
            owl:minCardinality 0 ;
            owl:onProperty nexus:refersToRisk ],
        [ a owl:Restriction ;
            owl:maxCardinality 1 ;
            owl:onProperty nexus:hasSeverity ],
        [ a owl:Restriction ;
            owl:maxCardinality 1 ;
            owl:onProperty nexus:source_uri ],
        [ a owl:Restriction ;
            owl:allValuesFrom xsd:string ;
            owl:onProperty nexus:source_uri ],
        [ a owl:Restriction ;
            owl:maxCardinality 1 ;
            owl:onProperty nexus:author ],
        [ a owl:Restriction ;
            owl:minCardinality 0 ;
            owl:onProperty nexus:hasStatus ],
        [ a owl:Restriction ;
            owl:maxCardinality 1 ;
            owl:onProperty nexus:hasImpact ],
        [ a owl:Restriction ;
            owl:minCardinality 0 ;
            owl:onProperty nexus:hasImpactOn ],
        [ a owl:Restriction ;
            owl:allValuesFrom nexus:RiskIncident ;
            owl:onProperty nexus:hasVariant ],
        [ a owl:Restriction ;
            owl:allValuesFrom nexus:Consequence ;
            owl:onProperty nexus:hasConsequence ],
        [ a owl:Restriction ;
            owl:minCardinality 0 ;
            owl:onProperty nexus:hasSeverity ],
        [ a owl:Restriction ;
            owl:maxCardinality 1 ;
            owl:onProperty nexus:hasImpactOn ],
        [ a owl:Restriction ;
            owl:allValuesFrom nexus:IncidentStatus ;
            owl:onProperty nexus:hasStatus ],
        [ a owl:Restriction ;
            owl:allValuesFrom nexus:Risk ;
            owl:onProperty nexus:refersToRisk ],
        [ a owl:Restriction ;
            owl:allValuesFrom nexus:Impact ;
            owl:onProperty nexus:hasImpact ],
        [ a owl:Restriction ;
            owl:minCardinality 0 ;
            owl:onProperty nexus:hasVariant ],
        nexus:Entity,
        nexus:RiskConcept ;
    skos:definition "An event occuring or occured which is a realised or materialised risk." ;
    skos:exactMatch <https://w3id.org/dpv/risk#Incident> ;
    skos:inScheme nexus:ai_risk .

nexus:Vocabulary a owl:Class ;
    rdfs:label "Vocabulary" ;
    rdfs:subClassOf [ a owl:Restriction ;
            owl:allValuesFrom xsd:string ;
            owl:onProperty nexus:version ],
        [ a owl:Restriction ;
            owl:allValuesFrom nexus:Documentation ;
            owl:onProperty nexus:hasDocumentation ],
        [ a owl:Restriction ;
            owl:minCardinality 0 ;
            owl:onProperty nexus:hasLicense ],
        [ a owl:Restriction ;
            owl:minCardinality 0 ;
            owl:onProperty nexus:version ],
        [ a owl:Restriction ;
            owl:maxCardinality 1 ;
            owl:onProperty nexus:hasLicense ],
        [ a owl:Restriction ;
            owl:maxCardinality 1 ;
            owl:onProperty nexus:version ],
        [ a owl:Restriction ;
            owl:allValuesFrom nexus:License ;
            owl:onProperty nexus:hasLicense ],
        [ a owl:Restriction ;
            owl:minCardinality 0 ;
            owl:onProperty nexus:hasDocumentation ],
        nexus:Entity ;
    skos:definition "A collection of terms, with their definitions and relationships." ;
    skos:inScheme nexus:common .

nexus:detectsRiskConcept a owl:ObjectProperty ;
    rdfs:label "detectsRiskConcept" ;
    rdfs:domain nexus:RiskControl ;
    rdfs:range nexus:RiskConcept ;
    owl:inverseOf nexus:isDetectedBy ;
    skos:definition "The property airo:detectsRiskConcept indicates the control used for detecting risks, risk sources, consequences, and impacts." ;
    skos:exactMatch airo:detectsRiskConcept ;
    skos:inScheme nexus:ai_risk .

nexus:RiskControl a owl:Class ;
    rdfs:label "RiskControl" ;
    rdfs:subClassOf [ a owl:Restriction ;
            owl:minCardinality 0 ;
            owl:onProperty nexus:isDefinedByTaxonomy ],
        [ a owl:Restriction ;
            owl:minCardinality 0 ;
            owl:onProperty nexus:detectsRiskConcept ],
        [ a owl:Restriction ;
            owl:maxCardinality 1 ;
            owl:onProperty nexus:isDefinedByTaxonomy ],
        [ a owl:Restriction ;
            owl:allValuesFrom nexus:RiskConcept ;
            owl:onProperty nexus:detectsRiskConcept ],
        [ a owl:Restriction ;
            owl:allValuesFrom nexus:RiskTaxonomy ;
            owl:onProperty nexus:isDefinedByTaxonomy ],
        nexus:Entity,
        nexus:RiskConcept ;
    skos:definition "A measure that maintains and/or modifies risk (and risk concepts)" ;
    skos:exactMatch airo:RiskControl ;
    skos:inScheme nexus:ai_risk .

nexus:author a owl:DatatypeProperty .

nexus:isProvidedBy a owl:ObjectProperty ;
    rdfs:label "isProvidedBy" ;
    rdfs:range nexus:AiProvider ;
    skos:definition "A relationship indicating the AI model has been provided by an AI model provider." ;
    skos:inScheme nexus:ai_system .

nexus:name a owl:DatatypeProperty ;
    rdfs:label "name" ;
    skos:definition "A text name of this instance.",
        "The official name of the benchmark." ;
    skos:inScheme nexus:ai_eval,
        nexus:common .

nexus:EuAiRiskCategory a owl:Class ;
    owl:unionOf ( <https://ibm.github.io/risk-atlas-nexus/ontology/EuAiRiskCategory#EXCLUDED> <https://ibm.github.io/risk-atlas-nexus/ontology/EuAiRiskCategory#PROHIBITED> <https://ibm.github.io/risk-atlas-nexus/ontology/EuAiRiskCategory#HIGH_RISK_EXCEPTION> <https://ibm.github.io/risk-atlas-nexus/ontology/EuAiRiskCategory#HIGH_RISK> <https://ibm.github.io/risk-atlas-nexus/ontology/EuAiRiskCategory#LIMITED_OR_LOW_RISK> ) ;
    linkml:permissible_values <https://ibm.github.io/risk-atlas-nexus/ontology/EuAiRiskCategory#EXCLUDED>,
        <https://ibm.github.io/risk-atlas-nexus/ontology/EuAiRiskCategory#HIGH_RISK>,
        <https://ibm.github.io/risk-atlas-nexus/ontology/EuAiRiskCategory#HIGH_RISK_EXCEPTION>,
        <https://ibm.github.io/risk-atlas-nexus/ontology/EuAiRiskCategory#LIMITED_OR_LOW_RISK>,
        <https://ibm.github.io/risk-atlas-nexus/ontology/EuAiRiskCategory#PROHIBITED> .

nexus:IncidentStatus a owl:Class ;
    rdfs:label "IncidentStatus" ;
    rdfs:subClassOf nexus:Entity ;
    skos:exactMatch <https://w3id.org/dpv#IncidentStatus> ;
    skos:inScheme nexus:ai_risk .

nexus:AiSystemType a owl:Class ;
    owl:unionOf ( <https://ibm.github.io/risk-atlas-nexus/ontology/AiSystemType#GPAI> <https://ibm.github.io/risk-atlas-nexus/ontology/AiSystemType#GPAI_OS> <https://ibm.github.io/risk-atlas-nexus/ontology/AiSystemType#PROHIBITED> <https://ibm.github.io/risk-atlas-nexus/ontology/AiSystemType#SCIENTIFIC_RD> <https://ibm.github.io/risk-atlas-nexus/ontology/AiSystemType#MILITARY_SECURITY> <https://ibm.github.io/risk-atlas-nexus/ontology/AiSystemType#HIGH_RISK> ) ;
    linkml:permissible_values <https://ibm.github.io/risk-atlas-nexus/ontology/AiSystemType#GPAI>,
        <https://ibm.github.io/risk-atlas-nexus/ontology/AiSystemType#GPAI_OS>,
        <https://ibm.github.io/risk-atlas-nexus/ontology/AiSystemType#HIGH_RISK>,
        <https://ibm.github.io/risk-atlas-nexus/ontology/AiSystemType#MILITARY_SECURITY>,
        <https://ibm.github.io/risk-atlas-nexus/ontology/AiSystemType#PROHIBITED>,
        <https://ibm.github.io/risk-atlas-nexus/ontology/AiSystemType#SCIENTIFIC_RD> .

nexus:AiEval a owl:Class ;
    rdfs:label "AiEval" ;
    rdfs:subClassOf [ a owl:Restriction ;
            owl:minCardinality 0 ;
            owl:onProperty nexus:isComposedOf ],
        [ a owl:Restriction ;
            owl:minCardinality 0 ;
            owl:onProperty nexus:hasUnitxtCard ],
        [ a owl:Restriction ;
            owl:minCardinality 0 ;
            owl:onProperty nexus:bestValue ],
        [ a owl:Restriction ;
            owl:minCardinality 0 ;
            owl:onProperty nexus:hasBenchmarkMetadata ],
        [ a owl:Restriction ;
            owl:allValuesFrom nexus:Dataset ;
            owl:onProperty nexus:hasDataset ],
        [ a owl:Restriction ;
            owl:minCardinality 0 ;
            owl:onProperty nexus:hasImplementation ],
        [ a owl:Restriction ;
            owl:allValuesFrom [ owl:intersectionOf ( [ owl:unionOf ( nexus:RiskConcept nexus:Term ) ] nexus:Risk ) ] ;
            owl:onProperty nexus:hasRelatedRisk ],
        [ a owl:Restriction ;
            owl:maxCardinality 1 ;
            owl:onProperty nexus:bestValue ],
        [ a owl:Restriction ;
            owl:allValuesFrom xsd:anyURI ;
            owl:onProperty nexus:hasUnitxtCard ],
        [ a owl:Restriction ;
            owl:allValuesFrom xsd:string ;
            owl:onProperty nexus:bestValue ],
        [ a owl:Restriction ;
            owl:minCardinality 0 ;
            owl:onProperty nexus:hasTasks ],
        [ a owl:Restriction ;
            owl:minCardinality 0 ;
            owl:onProperty nexus:hasLicense ],
        [ a owl:Restriction ;
            owl:maxCardinality 1 ;
            owl:onProperty nexus:hasLicense ],
        [ a owl:Restriction ;
            owl:allValuesFrom nexus:AiEval ;
            owl:onProperty nexus:isComposedOf ],
        [ a owl:Restriction ;
            owl:minCardinality 0 ;
            owl:onProperty nexus:hasRelatedRisk ],
        [ a owl:Restriction ;
            owl:allValuesFrom xsd:anyURI ;
            owl:onProperty nexus:hasImplementation ],
        [ a owl:Restriction ;
            owl:allValuesFrom xsd:string ;
            owl:onProperty nexus:hasTasks ],
        [ a owl:Restriction ;
            owl:allValuesFrom nexus:Documentation ;
            owl:onProperty nexus:hasDocumentation ],
        [ a owl:Restriction ;
            owl:allValuesFrom nexus:License ;
            owl:onProperty nexus:hasLicense ],
        [ a owl:Restriction ;
            owl:minCardinality 0 ;
            owl:onProperty nexus:hasDocumentation ],
        [ a owl:Restriction ;
            owl:minCardinality 0 ;
            owl:onProperty nexus:hasDataset ],
        [ a owl:Restriction ;
            owl:allValuesFrom nexus:BenchmarkMetadataCard ;
            owl:onProperty nexus:hasBenchmarkMetadata ],
        nexus:Entity ;
    skos:definition "An AI Evaluation, e.g. a metric, benchmark, unitxt card evaluation, a question or a combination of such entities." ;
    skos:exactMatch <https://www.w3.org/TR/vocab-dqv/Metric> ;
    skos:inScheme nexus:ai_eval .

nexus:RiskTaxonomy a owl:Class ;
    rdfs:label "RiskTaxonomy" ;
    rdfs:subClassOf [ a owl:Restriction ;
            owl:minCardinality 0 ;
            owl:onProperty nexus:hasDocumentation ],
        [ a owl:Restriction ;
            owl:allValuesFrom nexus:Documentation ;
            owl:onProperty nexus:hasDocumentation ],
        [ a owl:Restriction ;
            owl:maxCardinality 1 ;
            owl:onProperty nexus:hasLicense ],
        [ a owl:Restriction ;
            owl:minCardinality 0 ;
            owl:onProperty nexus:hasLicense ],
        [ a owl:Restriction ;
            owl:allValuesFrom xsd:string ;
            owl:onProperty nexus:version ],
        [ a owl:Restriction ;
            owl:allValuesFrom nexus:License ;
            owl:onProperty nexus:hasLicense ],
        [ a owl:Restriction ;
            owl:minCardinality 0 ;
            owl:onProperty nexus:version ],
        [ a owl:Restriction ;
            owl:maxCardinality 1 ;
            owl:onProperty nexus:version ],
        nexus:Entity ;
    skos:definition "A taxonomy of AI system related risks" ;
    skos:inScheme nexus:ai_risk .

nexus:isDefinedByVocabulary a owl:ObjectProperty ;
    rdfs:label "isDefinedByVocabulary" ;
    rdfs:range nexus:Vocabulary ;
    skos:definition "A relationship where a term or a term group is defined by a vocabulary" ;
    skos:inScheme nexus:common .

nexus:isPartOf a owl:DatatypeProperty ;
    rdfs:label "isPartOf" ;
    skos:definition "A relationship where an entity is part of another entity" ;
    skos:inScheme nexus:common .

nexus:version a owl:DatatypeProperty ;
    rdfs:label "version" ;
    skos:definition "The version of the entity embodied by a specified resource." ;
    skos:inScheme nexus:common .

nexus:Organization a owl:Class ;
    rdfs:label "Organization" ;
    rdfs:subClassOf [ a owl:Restriction ;
            owl:minCardinality 0 ;
            owl:onProperty nexus:grants_license ],
        [ a owl:Restriction ;
            owl:allValuesFrom nexus:License ;
            owl:onProperty nexus:grants_license ],
        [ a owl:Restriction ;
            owl:maxCardinality 1 ;
            owl:onProperty nexus:grants_license ],
        nexus:Entity ;
    skos:definition "Any organizational entity such as a corporation, educational institution, consortium, government, etc." ;
    skos:exactMatch <http://schema.org/Organization> ;
    skos:inScheme nexus:common .

nexus:License a owl:Class ;
    rdfs:label "License" ;
    rdfs:subClassOf [ a owl:Restriction ;
            owl:minCardinality 0 ;
            owl:onProperty nexus:version ],
        [ a owl:Restriction ;
            owl:allValuesFrom xsd:string ;
            owl:onProperty nexus:version ],
        [ a owl:Restriction ;
            owl:maxCardinality 1 ;
            owl:onProperty nexus:version ],
        nexus:Entity ;
    skos:definition "The general notion of a license which defines terms and grants permissions to users of AI systems, datasets and software." ;
    skos:exactMatch airo:License ;
    skos:inScheme nexus:common .

nexus:hasRelatedRisk a owl:ObjectProperty ;
    rdfs:label "hasRelatedRisk" ;
    rdfs:domain nexus:Any ;
    rdfs:range [ owl:intersectionOf ( [ owl:unionOf ( nexus:RiskConcept nexus:Term ) ] nexus:Risk ) ] ;
    skos:definition "A relationship where an entity relates to a risk" ;
    skos:inScheme nexus:ai_risk .

nexus:Documentation a owl:Class ;
    rdfs:label "Documentation" ;
    rdfs:subClassOf [ a owl:Restriction ;
            owl:minCardinality 0 ;
            owl:onProperty nexus:author ],
        [ a owl:Restriction ;
            owl:allValuesFrom xsd:string ;
            owl:onProperty nexus:author ],
        [ a owl:Restriction ;
            owl:allValuesFrom nexus:License ;
            owl:onProperty nexus:hasLicense ],
        [ a owl:Restriction ;
            owl:minCardinality 0 ;
            owl:onProperty nexus:hasLicense ],
        [ a owl:Restriction ;
            owl:maxCardinality 1 ;
            owl:onProperty nexus:author ],
        [ a owl:Restriction ;
            owl:maxCardinality 1 ;
            owl:onProperty nexus:hasLicense ],
        nexus:Entity ;
    skos:definition "Documented information about a concept or other topic(s) of interest." ;
    skos:exactMatch airo:Documentation ;
    skos:inScheme nexus:common .

nexus:Any a owl:Class ;
    rdfs:label "Any" ;
    skos:exactMatch linkml:Any ;
    skos:inScheme nexus:ai_risk .

nexus:RiskGroup a owl:Class ;
    rdfs:label "RiskGroup" ;
    rdfs:subClassOf [ a owl:Restriction ;
            owl:minCardinality 0 ;
            owl:onProperty nexus:broadMatch ],
        [ a owl:Restriction ;
            owl:allValuesFrom nexus:RiskTaxonomy ;
            owl:onProperty nexus:isDefinedByTaxonomy ],
        [ a owl:Restriction ;
            owl:minCardinality 0 ;
            owl:onProperty nexus:hasPart ],
        [ a owl:Restriction ;
            owl:minCardinality 0 ;
            owl:onProperty nexus:relatedMatch ],
        [ a owl:Restriction ;
            owl:allValuesFrom [ owl:intersectionOf ( [ owl:unionOf ( nexus:Risk nexus:RiskGroup ) ] nexus:Any ) ] ;
            owl:onProperty nexus:narrowMatch ],
        [ a owl:Restriction ;
            owl:allValuesFrom [ owl:intersectionOf ( [ owl:unionOf ( nexus:Risk nexus:RiskGroup ) ] nexus:Any ) ] ;
            owl:onProperty nexus:relatedMatch ],
        [ a owl:Restriction ;
            owl:allValuesFrom nexus:Risk ;
            owl:onProperty nexus:hasPart ],
        [ a owl:Restriction ;
            owl:minCardinality 0 ;
            owl:onProperty nexus:narrowMatch ],
        [ a owl:Restriction ;
            owl:minCardinality 0 ;
            owl:onProperty nexus:exactMatch ],
        [ a owl:Restriction ;
            owl:minCardinality 0 ;
            owl:onProperty nexus:closeMatch ],
        [ a owl:Restriction ;
            owl:allValuesFrom [ owl:intersectionOf ( [ owl:unionOf ( nexus:Risk nexus:RiskGroup ) ] nexus:Any ) ] ;
            owl:onProperty nexus:broadMatch ],
        [ a owl:Restriction ;
            owl:allValuesFrom [ owl:intersectionOf ( [ owl:unionOf ( nexus:Risk nexus:RiskGroup ) ] nexus:Any ) ] ;
            owl:onProperty nexus:exactMatch ],
        [ a owl:Restriction ;
            owl:allValuesFrom [ owl:intersectionOf ( [ owl:unionOf ( nexus:Risk nexus:RiskGroup ) ] nexus:Any ) ] ;
            owl:onProperty nexus:closeMatch ],
        [ a owl:Restriction ;
            owl:maxCardinality 1 ;
            owl:onProperty nexus:isDefinedByTaxonomy ],
        [ a owl:Restriction ;
            owl:minCardinality 0 ;
            owl:onProperty nexus:isDefinedByTaxonomy ],
        nexus:Entity,
        nexus:RiskConcept ;
    skos:definition "A group of AI system related risks that are part of a risk taxonomy." ;
    skos:inScheme nexus:ai_risk .

nexus:Term a owl:Class ;
    rdfs:label "Term" ;
    rdfs:subClassOf [ a owl:Restriction ;
            owl:allValuesFrom nexus:Term ;
            owl:onProperty nexus:hasParentDefinition ],
        [ a owl:Restriction ;
            owl:minCardinality 0 ;
            owl:onProperty nexus:hasSubDefinition ],
        [ a owl:Restriction ;
            owl:maxCardinality 1 ;
            owl:onProperty nexus:isDefinedByVocabulary ],
        [ a owl:Restriction ;
            owl:allValuesFrom nexus:Vocabulary ;
            owl:onProperty nexus:isDefinedByVocabulary ],
        [ a owl:Restriction ;
            owl:allValuesFrom nexus:Documentation ;
            owl:onProperty nexus:hasDocumentation ],
        [ a owl:Restriction ;
            owl:allValuesFrom nexus:Term ;
            owl:onProperty nexus:hasSubDefinition ],
        [ a owl:Restriction ;
            owl:allValuesFrom [ owl:intersectionOf ( [ owl:unionOf ( nexus:RiskConcept nexus:Term ) ] nexus:Risk ) ] ;
            owl:onProperty nexus:hasRelatedRisk ],
        [ a owl:Restriction ;
            owl:minCardinality 0 ;
            owl:onProperty nexus:hasParentDefinition ],
        [ a owl:Restriction ;
            owl:minCardinality 0 ;
            owl:onProperty nexus:isDefinedByVocabulary ],
        [ a owl:Restriction ;
            owl:minCardinality 0 ;
            owl:onProperty nexus:hasRelatedRisk ],
        [ a owl:Restriction ;
            owl:minCardinality 0 ;
            owl:onProperty nexus:hasDocumentation ],
        nexus:Entity ;
    skos:definition "A term and its definitions" ;
    skos:inScheme nexus:common .

nexus:isDefinedByTaxonomy a owl:ObjectProperty ;
    rdfs:label "isDefinedByTaxonomy" ;
    rdfs:range nexus:RiskTaxonomy ;
    skos:definition "A relationship where a risk or a risk group is defined by a risk taxonomy" ;
    skos:inScheme nexus:ai_risk .

nexus:hasDocumentation a owl:ObjectProperty ;
    rdfs:label "hasDocumentation" ;
    rdfs:range nexus:Documentation ;
    skos:definition "Indicates documentation associated with an entity." ;
    skos:inScheme nexus:common .

nexus:RiskConcept a owl:Class ;
    rdfs:label "RiskConcept" ;
    rdfs:subClassOf [ a owl:Restriction ;
            owl:minCardinality 0 ;
            owl:onProperty nexus:isDetectedBy ],
        [ a owl:Restriction ;
            owl:allValuesFrom nexus:RiskControl ;
            owl:onProperty nexus:isDetectedBy ],
        nexus:Entity ;
    skos:definition "An umbrella term for refering to risk, risk source, consequence and impact." ;
    skos:exactMatch airo:RiskConcept ;
    skos:inScheme nexus:ai_risk .

nexus:hasLicense a owl:ObjectProperty ;
    rdfs:label "hasLicense" ;
    rdfs:range nexus:License ;
    skos:definition "Indicates licenses associated with a resource" ;
    skos:inScheme nexus:common .

nexus:Risk a owl:Class ;
    rdfs:label "Risk" ;
    rdfs:subClassOf [ a owl:Restriction ;
            owl:maxCardinality 1 ;
            owl:onProperty nexus:tag ],
        [ a owl:Restriction ;
            owl:allValuesFrom nexus:RiskGroup ;
            owl:onProperty nexus:isPartOf ],
        [ a owl:Restriction ;
            owl:minCardinality 0 ;
            owl:onProperty nexus:tag ],
        [ a owl:Restriction ;
            owl:minCardinality 0 ;
            owl:onProperty nexus:detectsRiskConcept ],
        [ a owl:Restriction ;
            owl:maxCardinality 1 ;
            owl:onProperty nexus:phase ],
        [ a owl:Restriction ;
            owl:minCardinality 0 ;
            owl:onProperty nexus:descriptor ],
        [ a owl:Restriction ;
            owl:maxCardinality 1 ;
            owl:onProperty nexus:isDefinedByTaxonomy ],
        [ a owl:Restriction ;
            owl:allValuesFrom xsd:string ;
            owl:onProperty nexus:type ],
        [ a owl:Restriction ;
            owl:allValuesFrom [ owl:intersectionOf ( [ owl:unionOf ( nexus:Risk nexus:RiskGroup ) ] nexus:Any ) ] ;
            owl:onProperty nexus:exactMatch ],
        [ a owl:Restriction ;
            owl:allValuesFrom nexus:Action ;
            owl:onProperty nexus:hasRelatedAction ],
        [ a owl:Restriction ;
            owl:minCardinality 0 ;
            owl:onProperty nexus:relatedMatch ],
        [ a owl:Restriction ;
            owl:maxCardinality 1 ;
            owl:onProperty nexus:descriptor ],
        [ a owl:Restriction ;
            owl:allValuesFrom xsd:string ;
            owl:onProperty nexus:descriptor ],
        [ a owl:Restriction ;
            owl:minCardinality 0 ;
            owl:onProperty nexus:hasRelatedAction ],
        [ a owl:Restriction ;
            owl:minCardinality 0 ;
            owl:onProperty nexus:concern ],
        [ a owl:Restriction ;
            owl:minCardinality 0 ;
            owl:onProperty nexus:isPartOf ],
        [ a owl:Restriction ;
            owl:minCardinality 0 ;
            owl:onProperty nexus:exactMatch ],
        [ a owl:Restriction ;
            owl:minCardinality 0 ;
            owl:onProperty nexus:closeMatch ],
        [ a owl:Restriction ;
            owl:minCardinality 0 ;
            owl:onProperty nexus:narrowMatch ],
        [ a owl:Restriction ;
            owl:allValuesFrom [ owl:intersectionOf ( [ owl:unionOf ( nexus:Risk nexus:RiskGroup ) ] nexus:Any ) ] ;
            owl:onProperty nexus:broadMatch ],
        [ a owl:Restriction ;
            owl:minCardinality 0 ;
            owl:onProperty nexus:broadMatch ],
        [ a owl:Restriction ;
            owl:allValuesFrom [ owl:intersectionOf ( [ owl:unionOf ( nexus:Risk nexus:RiskGroup ) ] nexus:Any ) ] ;
            owl:onProperty nexus:closeMatch ],
        [ a owl:Restriction ;
            owl:allValuesFrom xsd:string ;
            owl:onProperty nexus:concern ],
        [ a owl:Restriction ;
            owl:allValuesFrom nexus:RiskConcept ;
            owl:onProperty nexus:detectsRiskConcept ],
        [ a owl:Restriction ;
            owl:allValuesFrom [ owl:intersectionOf ( [ owl:unionOf ( nexus:Risk nexus:RiskGroup ) ] nexus:Any ) ] ;
            owl:onProperty nexus:relatedMatch ],
        [ a owl:Restriction ;
            owl:maxCardinality 1 ;
            owl:onProperty nexus:isPartOf ],
        [ a owl:Restriction ;
            owl:minCardinality 0 ;
            owl:onProperty nexus:type ],
        [ a owl:Restriction ;
            owl:allValuesFrom xsd:string ;
            owl:onProperty nexus:phase ],
        [ a owl:Restriction ;
            owl:allValuesFrom xsd:string ;
            owl:onProperty nexus:tag ],
        [ a owl:Restriction ;
            owl:minCardinality 0 ;
            owl:onProperty nexus:isDefinedByTaxonomy ],
        [ a owl:Restriction ;
            owl:allValuesFrom nexus:RiskTaxonomy ;
            owl:onProperty nexus:isDefinedByTaxonomy ],
        [ a owl:Restriction ;
            owl:maxCardinality 1 ;
            owl:onProperty nexus:type ],
        [ a owl:Restriction ;
            owl:maxCardinality 1 ;
            owl:onProperty nexus:concern ],
        [ a owl:Restriction ;
            owl:allValuesFrom [ owl:intersectionOf ( [ owl:unionOf ( nexus:Risk nexus:RiskGroup ) ] nexus:Any ) ] ;
            owl:onProperty nexus:narrowMatch ],
        [ a owl:Restriction ;
            owl:minCardinality 0 ;
            owl:onProperty nexus:phase ],
        nexus:Entity,
        nexus:RiskConcept ;
    skos:definition "The state of uncertainty associated with an AI system, that has the potential to cause harms" ;
    skos:exactMatch airo:Risk ;
    skos:inScheme nexus:ai_risk .

nexus:Entity a owl:Class ;
    rdfs:label "Entity" ;
    rdfs:subClassOf [ a owl:Restriction ;
            owl:minCardinality 0 ;
            owl:onProperty nexus:dateCreated ],
        [ a owl:Restriction ;
            owl:allValuesFrom xsd:date ;
            owl:onProperty nexus:dateModified ],
        [ a owl:Restriction ;
            owl:maxCardinality 1 ;
            owl:onProperty nexus:description ],
        [ a owl:Restriction ;
            owl:minCardinality 0 ;
            owl:onProperty nexus:description ],
        [ a owl:Restriction ;
            owl:allValuesFrom xsd:string ;
            owl:onProperty nexus:name ],
        [ a owl:Restriction ;
            owl:allValuesFrom xsd:date ;
            owl:onProperty nexus:dateCreated ],
        [ a owl:Restriction ;
            owl:minCardinality 0 ;
            owl:onProperty nexus:url ],
        [ a owl:Restriction ;
            owl:maxCardinality 1 ;
            owl:onProperty nexus:url ],
        [ a owl:Restriction ;
            owl:minCardinality 0 ;
            owl:onProperty nexus:dateModified ],
        [ a owl:Restriction ;
            owl:allValuesFrom xsd:string ;
            owl:onProperty nexus:id ],
        [ a owl:Restriction ;
            owl:minCardinality 1 ;
            owl:onProperty nexus:id ],
        [ a owl:Restriction ;
            owl:maxCardinality 1 ;
            owl:onProperty nexus:id ],
        [ a owl:Restriction ;
            owl:allValuesFrom xsd:string ;
            owl:onProperty nexus:description ],
        [ a owl:Restriction ;
            owl:maxCardinality 1 ;
            owl:onProperty nexus:dateCreated ],
        [ a owl:Restriction ;
            owl:maxCardinality 1 ;
            owl:onProperty nexus:dateModified ],
        [ a owl:Restriction ;
            owl:maxCardinality 1 ;
            owl:onProperty nexus:name ],
        [ a owl:Restriction ;
            owl:minCardinality 0 ;
            owl:onProperty nexus:name ],
        [ a owl:Restriction ;
            owl:allValuesFrom xsd:anyURI ;
            owl:onProperty nexus:url ] ;
    skos:definition "A generic grouping for any identifiable entity." ;
    skos:exactMatch <http://schema.org/Thing> ;
    skos:inScheme nexus:common .
